update

metavarbaseequation.v
@@ -1,10 +1,19 @@
 (**
-Contents
-- Binding signatures with associated sytnax
-- Derivation of assignments
-- Models of a signature and their morphisms
-- Syntax as a model
-- Initiality
+Let L be the free Σ-monoid on Set^ℕ, with T the monad
+
+
+We are given a parallel pair Ly₀ ⇉ LV
+where V : ℕ → Set returns the set of metavariables with given arity.
+What we want is not just a weak coequaliser in Kl(T), in the sense that
+the output morphism is not unique, (induces a weak coequaliser in T-alg)
+but true coequaliser in Kl(T).
+Indeed, it seems we can prove that if t[ σ]ₘ = t[δ]ₘ, then σ and δ
+coincide on each metavariable that appears in t. From that we can deduce uniqueness.
+
+
+TODO: voir samemvar.json pour une tentative de preuve categorique
+que le cas same metavariable est correct
+
 *)
 
 Require Import Arith.
@@ -22,13 +31,20 @@ Require Import syntaxdb.
 Set Implicit Arguments.
 Unset Strict Implicit.
 Unset Printing Implicit Defensive.
+(*
+Maybe we could instead consider the following syntax:
+Inductive Z : Type :=
+  Var : nat -> Z
+| Op : nat -> list (nat, Z) -> Z
+| MVar : nat -> list Z -> Z
+So we could do it in Isabelle!
+ *)
 
 
   Theorem proj1 {A B}: A /\ B -> A.
   Proof.
     destruct 1; trivial.
     Defined.
-
   Theorem proj2 {A B}: A /\ B -> B.
   Proof.
     destruct 1; trivial.
@@ -95,15 +111,17 @@ destruct (a =m a') as [h|h].
 Defined.
 
 
-(*
 Instance deceq_option {A}{_ : EqDec A} : EqDec (option A).
 intros a a'.
 decide equality.
-Qed.
-*)
+Defined.
+
+Lemma deceq_eq_true {A}{_ : EqDec A} (a b: A) (eqb : a = b): a =m b = left eqb. 
+  Admitted.
 
 Lemma refl_deceq_true {A}{_ : EqDec A} (a : A) : a =m a = left eq_refl. 
-  Admitted.
+  apply deceq_eq_true.
+  Qed.
 (*
 Definition refl_deceq {A}{_ : EqDec A} (a : A) : a =m a. 
   cbn.
@@ -124,14 +142,112 @@ Fixpoint next_fv {S : signature} (z : Z S) : nat :=
   | Op op v => vec_max (vec_map (fun n x => next_fv x - n) v)
   end.
 
-Inductive In_fv {S } (p : nat) : Z S -> Type :=
+Inductive In_fv {S } (p : nat) : Z S -> Prop :=
   fv_var : In_fv p (Var _ p)
 | fv_op : forall (o : O S) (v : vec (Z S) (ar o)), In_fv_vec p v ->
                                                   In_fv p (Op o v)
-with In_fv_vec {S } (p : nat) : forall (l : list nat), vec (Z S) l -> Type :=
+with In_fv_vec {S } (p : nat) : forall (l : list nat), vec (Z S) l -> Prop :=
 | fv_hdV : forall a b l v, In_fv (p + a) b -> In_fv_vec p (ConsV a (lA := l) b v)
 | fv_tlV : forall a b l v, In_fv_vec p v -> In_fv_vec p (ConsV a (lA := l) b v).
 
+(*
+Fixpoint in_fv {S}(p : nat) (t : Z S) : Prop :=
+  match t with
+    Var _ q => q = p
+  | Op _ v => In_fv_vec p v
+    end.
+*)
+
+(*
+Lemma In_fv_Op {S} (p : nat) {o}(v : vec (Z S) (ar (s := S) o)) : In_fv p (Op o v) <-> In_fv_vec p v.
+  Admitted.
+*)
+
+
+
+Lemma In_fv_neq_subst {S} p (t : Z S) :
+  In_fv p t -> t [ fun n => if n =m p then Var _ (n + 1) else Var _ n ]ₛ <> t.
+Admitted.
+Lemma neq_subst_In_fv {S'} p (t : Z S') :
+        (* (forall f, f p <> p -> t [ fun n => Var _ (f n) ]ₛ <> t) -> *)
+        ( t [ fun n => Var _ (if n =m p then S n else n) ]ₛ <> t) ->
+        In_fv p t.
+  (*
+with neq_subst_In_fv_vec {S'} p (l : list nat)(v : vec (Z S') l) :
+  (* (forall f, f p <> p -> *)
+  (
+        (* vec_map (fun (n : nat) (b : Z S') => b [derivₙₛ (Var S') Z_ren n (fun n0 : nat => Var S' (f n0)) ]ₛ) v *)
+        vec_map (fun (n : nat) (b : Z S') => b [derivₙₛ (Var S') Z_ren n (fun n0 : nat => Var S' (if n0 =m p then S n0 else n0)) ]ₛ) v
+                 <> v
+  ) ->
+        In_fv_vec p v.
+*)
+  Admitted.
+Corollary neq_subst_In_fv_vec {S'} p (l : list nat)(v : vec (Z S') l) :
+  (* (forall f, f p <> p -> *)
+  (
+        (* vec_map (fun (n : nat) (b : Z S') => b [derivₙₛ (Var S') Z_ren n (fun n0 : nat => Var S' (f n0)) ]ₛ) v *)
+        vec_map (fun (n : nat) (b : Z S') => b [derivₙₛ (Var S') Z_ren n (fun n0 : nat => Var S' (if n0 =m p then S n0 else n0)) ]ₛ) v
+                 <> v
+  ) ->
+        In_fv_vec p v.
+Proof.
+  induction v.
+  - cbn.
+    contradiction.
+  - cbn.
+    Admitted.
+(*
+  {
+    destruct t.
+    - cbn.
+      intro h.
+      specialize (h (fun q => if p =m q then 1+q else q)).
+      revert h.
+      cbn.
+      rewrite refl_deceq_true.
+      cbn.
+      destruct (p =m n).
+      + subst.
+        constructor.
+      + intro h.
+        exfalso.
+        apply h.
+        * apply Nat.neq_succ_diag_l.
+        * reflexivity.
+    - cbn.
+      intro h.
+      assert (h' :
+                forall f : nat -> nat,
+      f p <> p ->
+       (vec_map (fun (n : nat) (b : Z S') => b [derivₙₛ (Var S') Z_ren n (fun n0 : nat => Var S' (f n0)) ]ₛ) v) <>
+       v
+).
+      admit.
+      constructor.
+      revert h'.
+      clear h.
+      induction v.
+      + cbn.
+        intro h.
+        exfalso.
+        apply (h S).
+        apply Nat.neq_succ_diag_l.
+        reflexivity.
+      + cbn.
+        Admitted.
+
+
+        speicalise
+      eapply neq_subst_In_fv_vec.
+      exact h'.
+  }
+  {
+    Guarded.
+    
+  }
+Admitted.
+*)
 
 Fixpoint Z_in_fv_subst_ext {S'} (f g : nat -> Z S')(z : Z S')
          (hfg : forall n, In_fv n z -> f n = g n) {struct z} :
@@ -201,6 +317,16 @@ Record msignature :=
 
 Existing Instance Om_dec.
 
+Definition extend_msig (V : msignature) (n : nat) : msignature :=
+  {| Om := option (Om V); arm := fun o => match o with None => n | Some o' => arm o' end |}.
+
+Notation "V +{ n }" := (extend_msig V n) (at level 30).
+
+Definition msignature_without (V : msignature) (o : Om V) : msignature :=
+  {| Om := { v | v <>m o}; arm := fun o' => arm (proj1_sig o') |}.
+
+Infix "\" := @msignature_without (at level 30).
+
 Coercion signature_from_msignature (V : msignature) :=
   {| O := Om V; ar := fun m => List.repeat 0 (arm m) |}.
 
@@ -252,9 +378,8 @@ Fixpoint vec_mk {A B} n (f : nat -> A -> B)(l : list A) : vec B l :=
 Definition vec_range0 {S}(m : model_data S)(n : nat) :=
 vec_mk 0 (fun n0 _ : nat => variables m n0) (List.repeat 0 n).
 
-Fixpoint vec_mk_ext {A B} n (f g : nat -> A -> B)(l : list A) :
-  (forall p a, p >= n -> f p a = g p a) -> vec_mk n f l = vec_mk n g l.
-  intro hfg.
+Fixpoint vec_mk_ext_exact {A B} n (f g : nat -> A -> B)(l : list A) :
+  (forall p a, p < n + length l -> p >= n -> f p a = g p a) -> vec_mk n f l = vec_mk n g l.
   refine
   (match l with
     nil => _
@@ -262,13 +387,43 @@ Fixpoint vec_mk_ext {A B} n (f g : nat -> A -> B)(l : list A) :
   end).
   reflexivity.
   cbn.
+  intro hfg.
   f_equal.
-  apply hfg.
-  constructor.
-  apply vec_mk_ext.
+  - apply hfg.
+    + lia.
+    + lia.
+  - apply vec_mk_ext_exact.
   intros.
   apply hfg.
   lia.
+  lia.
+  Qed.
+
+Lemma vec_mk_ext {A B} n (f g : nat -> A -> B)(l : list A) :
+  (forall p a, p >= n -> f p a = g p a) -> vec_mk n f l = vec_mk n g l.
+  intro H.
+  eapply vec_mk_ext_exact.
+  intros.
+  apply H.
+  assumption.
+Qed.
+
+Fixpoint vec_mk_eqf {A B} n (f : nat -> A -> B)(l : list A) :
+  vec_mk n f l = vec_mk 0 (fun p => f (n + p)) l.
+  Proof.
+  destruct l.
+  - reflexivity.
+  - cbn.
+    f_equal.
+    f_equal.
+    apply plus_n_O.
+    rewrite (vec_mk_eqf _ _ (S n)).
+    rewrite (vec_mk_eqf _ _ 1).
+    cbn.
+    apply vec_mk_ext.
+    intros.
+    f_equal.
+    lia.
   Qed.
 
 Fixpoint vec_nth_mk {A B}(default : B)(l : list A)(f : nat -> A -> B)(n m : nat) {struct l} :
@@ -465,7 +620,34 @@ n'a pas trop de fv
  *)
 
 
-
+Lemma assignation_fv {S n W} (a : an_assignation n (Z_model_data (S + W)%s))
+      (alaws : an_assignation_laws a) : forall p v, In_fv p (a v) -> In_fv_vec p v.
+intros p v in_pav.
+eapply neq_subst_In_fv_vec.
+apply In_fv_neq_subst in in_pav.
+intro h.
+apply in_pav.
+etransitivity.
+{ apply alaws. }
+f_equal.
+etransitivity; [|exact h].
+cbn.
+apply vec_map_ext.
+intros a' b'.
+cbn.
+unfold derivₛ.
+cbn.
+apply Z_subst_ext.
+intro q.
+apply derivₙₛ_ext_exact.
+- intros.
+  symmetry.
+  apply Z_ren_subst_eq.
+- intro hq.
+  cbn.
+  destruct (_ =m _); f_equal.
+  lia.
+  Qed.
 
 
 Definition id_assignation {S V} (m : model_data (S + V)%s) : assignation V m :=
@@ -521,6 +703,7 @@ Definition msubst {S : signature}{V : msignature} {W : msignature}(m : model_dat
   Defined.
 
 
+(* Fixpoint msubst' {S : signature}{V : msignature} {W : msignature}(m : model_data (S + W)%s) (f : assignation V m)(t : T S V)  : m. *)
 Fixpoint msubst' {S : signature}{V : msignature} {W : msignature}(m : model_data (S + W)%s) (f : assignation V m)(t : T S V)  : m.
   refine (
   match t with
@@ -551,9 +734,18 @@ induction t.
   apply msubst_eq.
   Qed.
 
+Lemma msubst'_id {S : signature}{V : msignature}  (t : T S V)  : t [ id_assignation (m := Z_model_data _)]ₘ = t.
+Admitted.
+
+Lemma msubst'_ren {S : signature}{V W : msignature}(m : model_data (S + W)%s)(a : assignation V m) f
+      (t : T S V) : t [ a ]ₘ [ fun x => variables m (f x) ] = 
+                       t [ fun x => Var _ (f x) ]ₛ [ a ]ₘ .
+Admitted.
 
 
-Definition assignation_raw_comp {S V W1 W2} {m : model_data (S + W2)%s}
+Definition assignation_raw_comp {S V W1 W2}
+           {m : model_data (S + W2)%s}
+           (* {m : model_data S} *)
   (a1 : assignation_raw V (ZModel (S + W1)%s)) 
   (a2 :assignation W1 m) : assignation_raw V m.
 intro o.
@@ -562,7 +754,17 @@ refine (t [ a2 ]ₘ).
 Defined.
 
 
-Definition assignation_comp {S V W1 W2} {m : model_data (S + W2)%s}
+(*
+Si V = { n }
+   W1 = {p}
+   W2 = {q}, alors
+a₁ ∘ a₂ (\vec{t}) = N(0,…,n-1)[ a₁ ]ₘ [ \vec{t} ]
+
+ *)
+(* push a1 along a2 *)
+Definition assignation_comp {S V W1 W2}
+           {m : model_data (S + W2)%s}
+           (* {m : model_data S} *)
   (a1 : assignation V (ZModel (S + W1)%s)) 
   (a2 :assignation W1 m) : assignation V m.
   apply mk_assignation.
@@ -571,23 +773,140 @@ Definition assignation_comp {S V W1 W2} {m : model_data (S + W2)%s}
   exact a2.
 Defined.
 
-Infix "∘c" := assignation_comp (at level 30).
+Infix "∘a" := assignation_comp (at level 30).
 
 Lemma assignation_comp_assoc {S V W1 W2 W3} {m : model_data (S + W3)%s}
   (a1 : assignation V (ZModel (S + W1)%s)) 
   (a2 :assignation W1 (ZModel (S + W2)%s))
   (a3 :assignation W2 m)
-  : a1 ∘c (a2 ∘c a3) = (a1 ∘c a2) ∘c a3.
+  : a1 ∘a (a2 ∘a a3) = (a1 ∘a a2) ∘a a3.
 Admitted.
 
 Lemma assignation_comp_idr {S V W} 
   (a1 : assignation V (Z_model_data (S + W)%s)) 
-   : a1 ∘c id_assignation (m := _) = a1.
+   : a1 ∘a id_assignation (m := _) = a1.
   Admitted.
 Lemma assignation_comp_idl {S V W} {m : model_data (S + W)%s}
   (a1 : assignation V m) 
-   : id_assignation (m := _) ∘c a1  = a1.
+   : id_assignation (m := _) ∘a a1  = a1.
   Admitted.
+
+(*
+  S : signature
+  eqO : forall x y : O S, {x = y} + {x <> y}
+  V : msignature
+  o : Om V
+  a : T S (V \ o)
+  o' : Om V
+  e : o' = o
+  ============================
+  an_assignation (arm o') (ZModel (S + V \ o)%s)
+*)
+Definition ass_instantiate1 {S}{V} {o o' : Om V}(a : T S (V \ o)) :
+  an_assignation (arm o') (ZModel (S + V \ o)%s).
+   apply mk_an_assignation.
+   exact a.
+Defined.
+
+Definition ass_instantiate2 {S}{V} {o o' : Om V}(a : T S (V \ o)) 
+  (eqo : o' <> o) :
+  an_assignation (arm o') (ZModel (S + V \ o)%s).
+   hnf.
+   unshelve eset (o'' := exist _ o' _ : O (V \ o) ).
+   { cbn.
+     apply neq_negb_deceq.
+     assumption.
+   }
+   change (arm o') with (arm o'').
+   apply TMVar.
+   Defined.
+Definition assignation_instantiate 
+           {S}
+  {V : msignature}
+  (o : Om V)
+  (a : T S (V \ o))
+  : assignation V (ZModel (S + V \ o)%s).
+ intro o'.
+ (* generalize (fun P => TMVar (S := S)(V := V \ o)(o := exist _ o' P)). *)
+ cbn.
+ destruct (o' =m o).
+ - apply ass_instantiate1.
+         (*
+   intro.
+   apply mk_an_assignation.
+*)
+   exact a.
+   (* apply mk_an_assignation. *)
+ - apply ass_instantiate2.
+   cbn.
+   (*
+   intro h.
+   refine( h _).
+*)
+   easy.
+   easy.
+   Defined.
+
+Definition assignation_omit {S V W} (m : model_data (S + W)%s)
+           (a : assignation  V m)
+           (o : Om V) :
+  assignation  (V \ o) m.
+Proof.
+  intros o' v.
+  cbn in o'.
+  apply (a (proj1_sig o')).
+  exact v.
+Defined.
+
+Lemma assignation_omit_laws {S V W} (m : model_data (S + W)%s)
+           (a : assignation  V m)
+           (alaws : assignation_laws a)
+           (o : Om V) :
+  assignation_laws (assignation_omit a (o := o)).
+Proof.
+  intros o' s v.
+  cbn.
+  unfold assignation_omit.
+  apply alaws.
+Qed.
+
+(* TODO: remove this lemma (it requires funext) *)
+Lemma assignation_ext {S V W} (m : model_data (S + W)%s)
+      (a b : assignation V m) :
+  (forall o v, a o v = b o v) -> a = b.
+Admitted.
+
+Lemma assignation_omit_postcomp {S V W1 W2} (m : model_data (S + W2)%s)
+           (a : assignation V (Z_model_data (S + W1)%s))
+           (a' : assignation W1 m)
+           (o : Om V) :
+  assignation_omit (a ∘a a') (o := o) = assignation_omit a (o := o) ∘a a'.
+apply assignation_ext.
+intros o' v.
+reflexivity.
+Qed.
+
+Definition assignation_incl {S V } (o : Om V) (m : model_data (S + V)%s) : assignation (V \ o) m.
+  apply assignation_omit.
+  apply id_assignation.
+Defined.
+
+
+
+
+
+(*
+Lemma instantiate_omit_eq {S V W} (m : model_data (S + W)%s)
+           (a : assignation  V m)
+           (o : Om V) 
+    (o' : Om V)(v : m ** (arm o')) : Type.
+  Check (assignation_omit a (o := o)).
+  Check ((assignation_comp (S := S)(W2 := _) _ (assignation_omit a (o := o)))).
+  refine (
+       a o' v = (assignation_comp (S := S) _ (assignation_omit a (o := o))) o' v).
+  apply assignation_instantiate.
+  assignation (S := S) (V \ o) m.
+*)
 
 
 (* Arguments Op [S V] o . *)
@@ -652,8 +971,19 @@ generalize (cass r1)(cass r2).
 apply assignation_comp.
 Defined.
 
+Infix "∘c" := (@candidate_comp _) (at level 30).
 
-Definition default_ass {V} : candidate V := mk_candidate (id_assignation (m := ZModel (S + V)%s)).
+
+Definition id_candidate {V} : candidate V := mk_candidate (id_assignation (m := ZModel (S + V)%s)).
+Definition id_candidate_ext {V} (n : nat) : candidate V.
+   refine {| cW := V +{ n } |} .
+   intros o v.
+   unshelve eapply (TMVar ).
+   exact (Some o).
+   exact v.
+   Defined.
+
+
 
 Fixpoint vec_fold {A B C : Type}{l : list A}(f : B -> C -> C) (c : C)(v : vec B l) : C :=
   match v with
@@ -696,9 +1026,9 @@ Fixpoint vec_fold2 {A B C D : Type}{l : list A}(f : C -> B -> D -> C) (c : C)(v1
 
 (*
 Equations make_unifier {V}(t u : T S V) : lazy_opt (candidate V) :=
-  make_unifier (Var _ n) (Var _ m) := mk_opt default_ass ( Nat.eqb n m) ;
+  make_unifier (Var _ n) (Var _ m) := mk_opt id_candidate ( Nat.eqb n m) ;
   make_unifier (Op (SOp o1) v1) (Op (SOp o2) v2) := _;
-  make_unifier _ _ := mk_opt default_ass false.
+  make_unifier _ _ := mk_opt id_candidate false.
 Next Obligation.
 Equations neg (b : bool) : bool :=
 neg true := _ ;
@@ -718,21 +1048,21 @@ Notation "'do' X <- A ; B" := (lazybind A (fun X => B)) (at level 200, X name, A
 Fixpoint make_unifier {V}(t u : T S V) {struct t }: lazy_opt (candidate V).
   refine 
   (match (t, u) with
-     (Var _ n, Var _ m) => mk_opt default_ass ( Nat.eqb n m)
+     (Var _ n, Var _ m) => mk_opt id_candidate ( Nat.eqb n m)
    | (Op o1 v1, Op o2 v2) => _
-   | _ => mk_opt default_ass false
+   | _ => mk_opt id_candidate false
     end).
   - clear t u.
     revert v1 v2.
     refine (match o1 with
               SOp o1' => match o2 with
                           SOp o2' => _
-                        | _ => fun _ _ => mk_opt default_ass false
+                        | _ => fun _ _ => mk_opt id_candidate false
                         end
-            | _ => fun _ _ => mk_opt default_ass false
+            | _ => fun _ _ => mk_opt id_candidate false
             end
            ).
-    refine (if eqO o1' o2' then _ else fun _ _ => mk_opt default_ass false).
+    refine (if eqO o1' o2' then _ else fun _ _ => mk_opt id_candidate false).
     intro v1.
     refine (match e with eq_refl => _ end).
     unshelve eapply (vec_fold2 _ _ v1).
@@ -746,28 +1076,28 @@ Fixpoint make_unifier {V}(t u : T S V) {struct t }: lazy_opt (candidate V).
       apply (candidate_comp r2).
       
     }
-    exact (retl default_ass).
+    exact (retl id_candidate).
     Abort. (* termination !! *)
 
 (* think of unifying t [ c ] and u *)
 Fixpoint make_unifier {V }(t : T S V) (c : candidate V) (u : T S (cW c)) {struct t }: lazy_opt (candidate V).
   refine 
   (match (t, u) with
-     (Var _ n, Var _ m) => mk_opt default_ass ( Nat.eqb n m)
+     (Var _ n, Var _ m) => mk_opt id_candidate ( Nat.eqb n m)
    | (Op o1 v1, Op o2 v2) => _
-   | _ => mk_opt default_ass false
+   | _ => mk_opt id_candidate false
     end).
   - clear t u.
     revert v1 v2.
     refine (match o1 with
               SOp o1' => match o2 with
                           SOp o2' => _
-                        | _ => fun _ _ => mk_opt default_ass false
+                        | _ => fun _ _ => mk_opt id_candidate false
                         end
-            | _ => fun _ _ => mk_opt default_ass false
+            | _ => fun _ _ => mk_opt id_candidate false
             end
            ).
-    refine (if eqO o1' o2' then _ else fun _ _ => mk_opt default_ass false).
+    refine (if eqO o1' o2' then _ else fun _ _ => mk_opt id_candidate false).
     intro v1.
     refine (match e with eq_refl => _ end).
     unshelve eapply (vec_fold2 _ _ v1).
@@ -787,7 +1117,7 @@ Fixpoint make_unifier {V }(t : T S V) (c : candidate V) (u : T S (cW c)) {struct
       apply (candidate_comp r2).
       
     }
-    exact (retl default_ass).
+    exact (retl id_candidate).
 *)
       Abort.
 
@@ -832,10 +1162,7 @@ Fixpoint in_mvar {S V} ov (t : T S V) {struct t} : Prop :=
 *)
               
 
-Definition msignature_without (V : msignature) (o : Om V) : msignature :=
-  {| Om := { v | v <>m o}; arm := fun o' => arm (proj1_sig o') |}.
 
-Infix "\" := @msignature_without (at level 30).
 
 
 Fixpoint remove_mvar {V} (t : T S V) ov (h : Notin_mvar ov t) { struct h }: T S (V \ ov)
@@ -864,6 +1191,34 @@ with remove_mvar_vec {V}(l : list nat)(v : vec (T S V) l) ov (h : Notin_mvar_vec
       eassumption.
   }
 Defined.
+
+Lemma remove_mvar_vec_assignation_incl 
+       {V}(l : list nat)(v : vec (T S V) l) ov (h : Notin_mvar_vec ov v) : 
+   vec_map (fun _ x => x [ assignation_incl (o := ov) (m := Z_model_data _)]ₘ) (remove_mvar_vec h) = v. 
+  Admitted.
+
+Lemma Notin_mvar_op {V}  (o : O S) ov v (t := (Op (S := S + V)%s (SOp (V := V) o) v))(h : Notin_mvar ov t) :
+  Notin_mvar_vec ov v.
+  Admitted.
+
+(*
+Lemma Notin_mvar_irrelevant   {V : msignature}(o :  Om V) (t : T S V)(h h' : Notin_mvar o t) :
+  h = h'.
+  Admitted.
+*)
+Lemma Notin_mvar_op_eta {V}  (o : O S) ov v (t := (Op (S := S + V)%s (SOp (V := V) o) v))(h : Notin_mvar ov t) :
+  h = NMsop (Notin_mvar_op h).
+  Admitted.
+
+
+
+Lemma remove_mvar_op {V}  (o : O S) ov v (t := (Op (S := S + V)%s (SOp (V := V) o) v))(h : Notin_mvar ov t)
+      : remove_mvar h = Op (S := S + _)%s (SOp (V := _) o) (remove_mvar_vec (Notin_mvar_op h)).
+  assert (heq := Notin_mvar_op_eta h).
+  rewrite heq at 1.
+  cbn.
+  reflexivity.
+Qed.
 
 (*
 Fixpoint remove_mvar {V} (t : T S V) { struct t} : forall o' (h : notin_mvar o' t), T S (V \ o').
@@ -949,60 +1304,6 @@ Defined.
 
 
 
-(*
-  S : signature
-  eqO : forall x y : O S, {x = y} + {x <> y}
-  V : msignature
-  o : Om V
-  a : T S (V \ o)
-  o' : Om V
-  e : o' = o
-  ============================
-  an_assignation (arm o') (ZModel (S + V \ o)%s)
-*)
-Definition ass_instantiate1 {V} {o o' : Om V}(a : T S (V \ o)) :
-  an_assignation (arm o') (ZModel (S + V \ o)%s).
-   apply mk_an_assignation.
-   exact a.
-Defined.
-
-Definition ass_instantiate2 {V} {o o' : Om V}(a : T S (V \ o)) 
-  (eqo : o' <> o) :
-  an_assignation (arm o') (ZModel (S + V \ o)%s).
-   hnf.
-   unshelve eset (o'' := exist _ o' _ : O (V \ o) ).
-   { cbn.
-     apply neq_negb_deceq.
-     assumption.
-   }
-   change (arm o') with (arm o'').
-   apply TMVar.
-   Defined.
-Definition assignation_instantiate 
-  {V : msignature}
-  (o : Om V)
-  (a : T S (V \ o))
-  : assignation V (ZModel (S + V \ o)%s).
- intro o'.
- (* generalize (fun P => TMVar (S := S)(V := V \ o)(o := exist _ o' P)). *)
- cbn.
- destruct (o' =m o).
- - apply ass_instantiate1.
-         (*
-   intro.
-   apply mk_an_assignation.
-*)
-   exact a.
-   (* apply mk_an_assignation. *)
- - apply ass_instantiate2.
-   cbn.
-   (*
-   intro h.
-   refine( h _).
-*)
-   easy.
-   easy.
-   Defined.
 
 Definition candidate_instantiate {V} {o : Om V}(a : T S (V \ o)) : candidate V.
  refine  {| cW := V \ o; cass := _|}.
@@ -1101,6 +1402,46 @@ Definition candidate_replace {V} {o : Om V}(n : nat)(a : T S (V [ o := n ])) : c
  refine  {| cW := V [ o := n]; cass := _|}.
  eapply (assignation_replace).
  exact a.
+Defined.
+
+(*
+Definition assignation_replace'
+  {V : msignature}
+  (o : Om V)
+  (n : nat)
+  (a : T S (V +{ n } \ Some o ))
+  : assignation V (ZModel (S + (V +{ n } \ Some o ))%s).
+ intro o'.
+ cbn.
+ eapply candidate_instantiate.
+ generalize (TMVar (S := S)(V := (V \ o +{ n } ) ) ).
+ cbn.
+ destruct (o' =m o).
+ - intro.
+   eapply mk_an_assignation.
+   exact a.
+ - intro h.
+   exact h. 
+   Defined.
+*)
+
+
+Definition candidate_replace' {V} {o : Om V}(n : nat)(a : T S ((V +{n} \ Some o) )) : candidate V.
+  unshelve refine (_ ∘c _).
+  apply id_candidate_ext.
+  exact n.
+  cbn.
+  eapply candidate_instantiate.
+  exact a.
+Defined.
+
+Definition TMVar_replaced' {V : msignature}(ov : Om V)(n : nat)(v : (T S (V +{ n } \ Some ov)) ** n) :
+  T S (V +{ n } \ Some ov).
+  unshelve refine (TMVar (V := V +{ n } \ Some ov)(o :=  exist _ None _) _).
+  - cbn.
+    easy.
+  - cbn.
+    exact v.
 Defined.
 
 Fixpoint Notin_mvar_msubst {V}{ov : Om V} t u (ht : Notin_mvar ov t) {struct ht}:
@@ -1224,7 +1565,7 @@ Lemma assignation_comp_msubst'
  {V W1 W2 : msignature} {m : model_data (S + W2)%s}
   (a : assignation V (ZModel (S + W1)%s)) (a' : assignation W1 m) t :
   t [ a ]ₘ [ a' ]ₘ =
-  t [ a ∘c a' ]ₘ. 
+  t [ a ∘a a' ]ₘ. 
   Admitted.
 
 (*
@@ -1289,6 +1630,7 @@ Inductive Vec_In (A B : Type) (b : B) : forall (l : list A), vec B l -> Prop :=
 | InV_tl : forall a b' l v, @Vec_In A B b _ v -> @Vec_In A B b _ (ConsV a (lA := l) b' v).
 
 Open Scope bool_scope.
+(* Maybe I only need an inversion on Vec_In Cons ? *)
 Fixpoint vec_in (A B : Type){eqb : EqDec B} (b : B) (l : list A)(v : vec B l) : bool :=
   match v with
     NilV => false
@@ -1300,11 +1642,6 @@ Lemma Vec_In_in
       (A B : Type){eqb : EqDec B} (b : B) (l : list A)(v : vec B l) : vec_in b v <-> Vec_In b v.
 Admitted.
 
-Fixpoint distinct (A B : Type){eqb : EqDec B} (l : list A)(v : vec B l) : bool :=
-  match v with
-    NilV => true
-  | ConsV a b' v => (negb (vec_in b' v)) && distinct v
-    end.
 
 Fixpoint inverse_vec_value {A : Type}(l : list A)(v : vec nat l) p n (hn : Vec_In n v) {struct hn} :
   inverse_vec p v n = p + inverse_vec 0 v n.
@@ -1341,6 +1678,104 @@ destruct hn.
  apply inverse_vec_is_inverse.
  assumption.
  Qed.
+
+Lemma vec_hd_tl_eta {A}{B}{a : A}{lA} (v : vec B (a :: lA)) : v = ConsV a (vec_hd v)  (vec_tl v).
+  Admitted.
+Lemma vec_map_ext_In {A B C} (f g :  B -> C)(l : list A)(v : vec B l)
+      (eq_fg : forall (b : B), Vec_In b v -> f b = g b) :
+  vec_map (fun _ => f) v =
+  vec_map (fun _ => g) v.
+  Admitted.
+Fixpoint distinct (A B : Type){eqb : EqDec B} (l : list A)(v : vec B l) : bool :=
+  match v with
+    NilV => true
+  | ConsV a b' v => (negb (vec_in b' v)) && distinct v
+    end.
+(* TODO: see if this can be used instead of the previous lemma *)
+Fixpoint map_inverse_vec_mk {A B : Type}(l : list A)(f : nat -> B)(v : vec nat l) (d : distinct v) {struct v} :
+      vec_map (fun _ x => f (inverse_vec 0 v x)) v = vec_mk 0 (fun n _ => f n) l.
+ destruct v.
+- cbn.
+  reflexivity.
+- cbn.
+  rewrite refl_deceq_true.
+  f_equal.
+  cbn.
+  cbn in d.
+  apply andb_prop in d.
+  destruct d as [d1 d2].
+  rewrite vec_mk_eqf.
+  cbn.
+  etransitivity; revgoals.
+  apply (map_inverse_vec_mk _ _ _ _ v d2).
+  apply vec_map_ext_In.
+  intros b inb.
+  destruct (b =m n).
+  + exfalso.
+    subst b.
+    rewrite <- Vec_In_in in inb.
+    rewrite inb in d1.
+    cbn in d1.
+    discriminate d1.
+  + rewrite inverse_vec_value.
+    reflexivity.
+    exact inb.
+Qed.
+Fixpoint inverse_vec_lt {A : Type }{l : list A} (v : vec nat l) (n : nat) (inn : Vec_In n v) {struct inn }:
+  v ̅ ¹ n < length l.
+Proof.
+  destruct inn.
+  - cbn.
+    rewrite refl_deceq_true.
+    lia.
+  - cbn.
+    destruct (n =m b').
+    lia.
+    rewrite inverse_vec_value;[|assumption].
+    cbn.
+    apply lt_n_S.
+    apply inverse_vec_lt.
+    assumption.
+Qed.
+
+Fixpoint vec_nth_default {A B : Type} (b b' :B) (l : list A) (v :  vec B l) (n : nat) {struct v} :
+  n < length l ->
+  vec_nth b v n = vec_nth b' v n.
+Proof.
+  destruct v.
+  - cbn.
+    lia.
+  - cbn.
+    destruct n.
+    + reflexivity.
+    + intro.
+      apply vec_nth_default.
+      lia.
+Qed.
+
+Corollary inverse_vec_is_inverse2 {A B : Type}(l : list A)(v : vec nat l)(v' : vec B l) (d : distinct v) b :
+      vec_map (fun _ x => vec_nth (b x) v' (inverse_vec 0 v x)) v = v'.
+  destruct l.
+  - 
+    refine (match v' with NilV => _ end).
+    refine (match v with NilV => _ end).
+    reflexivity.
+  - set (n0 := vec_hd v).
+    enough ( h : vec_map (fun (_ : A) (x : nat) => vec_nth (b x) v' ((v) ̅ ¹ x)) v
+           = vec_map (fun (_ : A) (x : nat) => vec_nth (b n0) v' ((v) ̅ ¹ x)) v).
+    {
+      etransitivity.
+      apply h.
+      etransitivity.
+      eapply (map_inverse_vec_mk _ (v := v) d).
+      apply vec_mk_nth0.
+    }
+    apply vec_map_ext_In.
+    intros b' inb'.
+    apply vec_nth_default.
+    apply inverse_vec_lt.
+    assumption.
+  Qed.
 
 Fixpoint vec_nth_map {A B C} (l : list A)(v : vec B l)(f : A -> B -> C)p (hp : p < length l) a b c {struct v}: 
   vec_nth c (vec_map f v) p = f (List.nth p l a) (vec_nth b v p).
@@ -1432,7 +1867,21 @@ Inductive vec_common_pos {B} : forall (n0 : nat) (v0 : B ** n0) (n1 : nat)(v1 v1
                                       b <> b' ->
                                 vec_common_pos v0 (n1 := 1 + n1)(ConsV 0 b v1)(ConsV 0 b' v1')
 
+
 .
+Inductive vec_common_val {B}{n1}(v1 : B ** n1) : forall  n1' (v1': B ** n1') (n0 : nat) (v0 : B ** n0), Type
+  :=
+  CVNil : @vec_common_val B n1 v1 0 NilV 0 NilV
+| CVIn : forall n0 (v0 : B ** n0) n1' (v1' : B ** n1') b,
+    vec_common_val v1 v0 v1' ->
+    Vec_In b v1 -> vec_common_val v1 (n1' := 1 + n1')(ConsV 0 b v1')(n0 := 1 + n0) (ConsV 0 b v0) 
+| CVNotIn : forall n0 (v0 : B ** n0) n1' (v1' : B ** n1') b,
+    vec_common_val v1 v0 v1' ->
+    ~ Vec_In b v1 -> vec_common_val v1 (n1' := 1 + n1')(ConsV 0 b v1') v0. 
+
+Lemma vec_common_pos_val {B}{n0}(v0 : B ** n0) {n1}( v1 v1' : B ** n1) :
+  vec_common_pos v0 v1 v1' -> vec_common_val v1 v1' v0.
+  Admitted.
 
 (*
 Definition replace_mvar {V} (o : Om V)(n := arm o)(v : nat ** n)(W :=
@@ -1446,7 +1895,7 @@ Definition replace_mvar {V} (o : Om V)(n := arm o)(v : nat ** n)(W :=
   cbn.
   intro v'.
   apply (TMVar (V := W)(o := o')).
-  cbn.
+
   destruct (o =m o').
   Cane peut pas marcher
   - exact (vec_mk 0 (fun x _ => Var _ x) (List.repeat 0 _)).
@@ -1471,6 +1920,26 @@ I would need to prove something before, like if the input unifies things, then t
 also does.
 
  ************* *)
+Lemma neq_Some {A}{o1 o2 : A} (eo : o1 <> o2) : Some o2 <> Some o1.
+  congruence.
+Qed.
+
+(*
+Lemma neq_Some_eq_dec {A} {eqA : EqDec A}{o1 o2 : A} (eo : o1 <> o2) : (Some o2 =m Some o1) = right (neq_Some eo).
+Admitted.
+*)
+(*
+
+Goal forall V n0 o1 o2 (eo : o1 <> o2), (fun v : Om (V +{ n0}) => is_true (v <>m Some o1)) (Some o2).
+intros.
+cbn beta.
+apply neq_negb_deceq.
+apply Some_neq.
+right.
+eapply right.
+cbn.
+*)
+
 
 (* thanks to applyass_spec,
    we can always assume that the input is the identity *)
@@ -1480,22 +1949,40 @@ Inductive unifier_spec  : forall V, T S V -> T S V -> forall (acc : candidate V)
     @unifier_spec_vec V _ v1 v2 c1 c2
     ->
     @unifier_spec V (Op (S := S + V)%s (SOp o) v1) (Op (S := S + V)%s (SOp o) v2) c1 c2
-                                     (* TODO correct *)
-                  (* TODO: remove *)
-| mvar_spec : forall V o (v1 v2 : vec nat (ar (s := S + V)%s(SMVar o))) c,
-    v1 = v2 ->
-    (* TODO: apply c to o *)
-    @unifier_spec V (Op (S := S + V)%s (SMVar o) (vec_map (fun _ => Var _)v1))
-                 (Op (S := S + V)%s (SMVar o) (vec_map (fun _ => Var _)v2))
-                 c c
 | same_mvar : forall V o (v1 v2 : vec nat (ar (s := S + V)%s(SMVar o))) 
                 n0 v0, vec_common_pos (n0 := n0) v0 v1 v2 ->
                        distinct v1 -> distinct v2 ->
                        @unifier_spec V (Op (S := S + V)%s (SMVar o) (vec_map (fun _ => Var _)v1))
                                      (Op (S := S + V)%s (SMVar o) (vec_map (fun _ => Var _)v2))
-                                     default_ass
-                                     (candidate_replace (o := o)
-                                                (TMVar_replaced (vec_map (fun _ => Var _)v0)[ fun k =>  Var _ (v1 ̅ ¹ k) ]ₛ))
+                                     id_candidate
+                                     (candidate_replace' (o := o)
+                                                (TMVar_replaced' (vec_map (fun _ => Var _)v0)[ fun k =>  Var _ (v1 ̅ ¹ k) ]ₛ))
+| different_mvar : forall V o1 o2 (neq_o12 : o1 <> o2)(v1 : vec nat (ar (s := S + V)%s(SMVar o1)))
+                     (v2 : vec nat (ar (s := S + V)%s(SMVar o2)))
+                     n0 v0
+                    (o2' := exist _ (Some o2) (neq_negb_deceq (neq_Some neq_o12)) : Om (V +{ n0 } \ Some o1))
+               , vec_common_val (n0 := n0) v1 v2 v0 ->
+                       (* distinct v1 -> distinct v2 -> *)
+                       @unifier_spec V (Op (S := S + V)%s (SMVar o1) (vec_map (fun _ => Var _)v1))
+                                     (Op (S := S + V)%s (SMVar o2) (vec_map (fun _ => Var _)v2))
+                                     id_candidate
+                                     (
+                                       id_candidate_ext n0
+                                        ∘c candidate_instantiate (V := V +{ n0 }) (o := Some o1)
+                                          (TMVar (V := V +{ n0 } \ Some o1)(o := exist _ None eq_refl)
+                                                (vec_map (fun _ p => Var _ (v1 ̅ ¹ p)) v0))
+                                        ∘c candidate_instantiate (V := V +{ n0 } \ Some o1)
+                                          (o := o2') 
+                                          (TMVar (V := V +{ n0 } \ Some o1 \ o2')(o := exist _ (exist _ None eq_refl) eq_refl)
+                                          (vec_map (fun _ p => Var _ (v2 ̅ ¹ p)) v0))
+                                     )
+                                     
+                                     (* (candidate_comp (r1 :=  *)
+                                     
+                                     (* candidate_replace (o := o1) *)
+                                     (*            (TMVar_replaced (vec_map (fun _ => Var _)v0)[ fun k =>  Var _ (v1 ̅ ¹ k) ]ₛ)) *)
+                                     (* (candidate_instantiate (o := o2) _) *)
+                                     (* ) *)
 
 (*
 1. m1[x1,..,xn] = m1[y1,..,yn]
@@ -1510,9 +1997,9 @@ When metavariables are different, you can reorder those parameters in 2. but not
 
 
 
-| applyass_spec : forall V t u c cf, @unifier_spec _ (t [ cass c ]ₘ) (u [ cass c ]ₘ) default_ass cf
+| applyass_spec : forall V t u c cf, @unifier_spec _ (t [ cass c ]ₘ) (u [ cass c ]ₘ) id_candidate cf
                                             -> 
-                                              @unifier_spec V t u c (candidate_comp (r1 := c) cf)
+                                              @unifier_spec V t u c (c ∘c cf)
 (* M[k1,...,kₙ] = t
 then M [u1,...,uₙ] = t [kᵢ ↦ uᵢ]
 Let us assume to start with that k1,...,kn = 0,..,n-1
@@ -1520,7 +2007,7 @@ and maybe add an instantiation case that replace M[k1, ..., kn] with N[0,..,m]?
  *)
    (* ce qu il faut faire c'est construire un inverse (en tant que nat -> nat) de v (vecteur d'entiers) *)
    (* et ensuite mk_assignation de t[v^-1] *)
-| instantiation_spec : forall V (c0 := default_ass) o (n := arm o) (v : nat ** n)(* (v : nat ** arm o) *) (u : T S V)
+| instantiation_spec : forall V (c0 := id_candidate) o (n := arm o) (v : nat ** n)(* (v : nat ** arm o) *) (u : T S V)
                          (hu : Notin_mvar o u)
   (hufv : forall n, In_fv n u -> Vec_In n v), (* next_fv u <= n *)
                           @unifier_spec V
@@ -1530,25 +2017,14 @@ and maybe add an instantiation case that replace M[k1, ..., kn] with N[0,..,m]?
                                             (candidate_instantiate (remove_mvar hu [ fun k =>  Var _ (v ̅ ¹ k) ]ₛ))
                                             (* (mk_assignation (m := ZModel (S + V \ o)) ) *)
                                                            (* missing case: instantiation *)
-(*
-M[x1, ..., xn]
-introduce new metavar N
-M[x1,...,xn] ↦ N[0,.., max(xn)-1] 
-*)
-                                            (*
-| normalise_mvar : forall V c0 o (n := arm o)(v : nat ** n) (u : T S V)
-                     (c' := {| cW := {| Om := Om V;
-                                       arm := fun o' => if o =m o' then arm o' else arm o'
-                                     |} ;
-                     cass := normalise_mvar_vec v
-                     |}),
-    @unifier_spec V (Op (S := S + V)%s (SMVar o) (vec_map (fun _ => Var _) v)) u
-                  c0 c'
-*)
+| sym_spec : forall V c0 t u c, @unifier_spec V t u c0 c -> unifier_spec u t c0 c
+(* Inductive unifier_spec  : forall V, T S V -> T S V -> forall (acc : candidate V) , candidate V -> Prop := *)
+
 with unifier_spec_vec : forall V (l : list nat), vec (T S V) l -> vec (T S V) l -> forall c : candidate V, candidate V -> Prop :=
-  NilV_spec : forall V c, @unifier_spec_vec V _ NilV NilV c default_ass
-| ConsV_spec : forall V n l t1 t2 (v1 v2 : vec (T S V) l) c1  c1' c2, @unifier_spec_vec V _ v1 v2 c1 c1' ->
+  NilV_spec : forall V c, @unifier_spec_vec V _ NilV NilV c c
+| ConsV_spec : forall V n l t1 t2 (v1 v2 : vec (T S V) l) c1  c1' c2, 
                                                           (* do we need to take n into account? I think n *)
+                                        @unifier_spec_vec V _ v1 v2 c1 c1' ->
                                         @unifier_spec V t1 t2 c1' c2 ->
                                         @unifier_spec_vec V _ (ConsV n t1 v1) (ConsV n t2 v2) c1
                                                          c2.
@@ -1579,11 +2055,36 @@ Lemma assignation_replace_TMVar_replaced
   contradiction.
 Qed.
 
-Lemma vec_map_ext_In {A B C} (f g :  B -> C)(l : list A)(v : vec B l)
-      (eq_fg : forall (b : B), Vec_In b v -> f b = g b) :
-  vec_map (fun _ => f) v =
-  vec_map (fun _ => g) v.
+(*
+Lemma assignation_replace'_TMVar_replaced'
+  {V : msignature}
+  (o : Om V)
+  (n : nat)
+  (a : T S (V [ o := n ]))
+  (v : T S (V [ o := n ]) ** (arm o))
+  
+  : assignation_replace' a v =
+      a [ vec_to_ren (m := Z_model_data _) v].
+  unfold assignation_replace.
+  generalize (TMVar (S := S)(V := V[o := n])(o:=o)).
+  cbn.
+  destruct (o =m o).
+  reflexivity.
+  contradiction.
+Qed.
+*)
+
+(*
+Inductive Vec_In' (A B : Type) (a : A)(b : B) : forall (l : list A), vec B l -> Prop :=
+  InV_hd' : forall (l :list A) v, @Vec_In' A B a b _ (ConsV a (lA := l) b v)
+| InV_tl' : forall a' b' l v, @Vec_In' A B a b _ v -> @Vec_In' A B _ b  _ (ConsV a' (lA := l) b' v).
+
+Lemma vec_map_ext_In' {A B C} (f g : A -> B -> C)(l : list A)(v : vec B l)
+      (eq_fg : forall (a : A)(b : B), Vec_In' a b v -> f a b = g a b) :
+  vec_map f v =
+  vec_map g v.
   Admitted.
+*)
 
      (* M(0,1,2,4) M(2,1,0,4)
 v0 = [1, 4]
@@ -1629,13 +2130,24 @@ Lemma vec_map_vecn {B C}(f : nat -> B -> C) n (v : B ** n) :
 vec_map f v = vec_map (fun _ b => f 0 b) v.
 Admitted.
 
+Lemma commonVal_Vec_In1 {B} n0 (v0 : B ** n0)n1 n1' (v1 : B ** n1)(v1' : B ** n1')(h : vec_common_val v1 v1' v0)
+      b (inb : Vec_In b v0) : Vec_In b v1.
+  Admitted.
+Lemma commonVal_Vec_In2 {B} n0 (v0 : B ** n0)n1 n1' (v1 : B ** n1)(v1' : B ** n1')(h : vec_common_val v1 v1' v0)
+      b (inb : Vec_In b v0) : Vec_In b v1'.
+  Admitted.
+
 
 Lemma commonPos_Vec_In1 {B} n0 (v0 : B ** n0)n1 (v1 v1' : B ** n1)(h : vec_common_pos v0 v1 v1')
       b (inb : Vec_In b v0) : Vec_In b v1.
-  Admitted.
+  apply vec_common_pos_val in h.
+  eapply commonVal_Vec_In1; eassumption.
+  Qed.
 Lemma commonPos_Vec_In2 {B} n0 (v0 : B ** n0)n1 (v1 v1' : B ** n1)(h : vec_common_pos v0 v1 v1')
       b (inb : Vec_In b v0) : Vec_In b v1'.
-  Admitted.
+  apply vec_common_pos_val in h.
+  eapply commonVal_Vec_In2; eassumption.
+  Qed.
 
 Lemma commonPos_Vec_inverse  n0 (v0 : nat ** n0)n1 (v1 v1' : nat ** n1)(h : vec_common_pos v0 v1 v1')
       b (d1 : distinct v1)(d2 : distinct v1')(inb : Vec_In b v0) : v1 ̅ ¹ b = v1' ̅ ¹ b.
@@ -1690,6 +2202,184 @@ Lemma commonPos_Vec_inverse  n0 (v0 : nat ** n0)n1 (v1 v1' : nat ** n1)(h : vec_
     (* I need the distinct hypothesis *)
       Qed.
 
+(*
+         (derivₙₛ (Var (S + (V +{ n0}) \ Some o)%s) Z_ren a
+            (vec_to_ren
+               (vec_map
+                  (fun _ : nat =>
+                   msubst'
+                     (fun o' : option (Om V) =>
+                      match deceq_option o' (Some o) with
+                      | left _ =>
+                          ass_instantiate1
+                            (Op
+                               (SMVar (exist (fun v : option (Om V) => negb (deceq_option v (Some o))) None eq_refl))
+                               (vec_map
+                                  (fun a0 b : nat =>
+                                   derivₙₛ (Var (S + (V +{ n0}) \ Some o)%s) Z_ren a0
+                                     (fun k : nat => Var (S + (V +{ n0}) \ Some o)%s ((v1) ̅ ¹ k)) b) v0))
+                      | right b =>
+                          ass_instantiate2
+                            (Op
+                               (SMVar (exist (fun v : option (Om V) => negb (deceq_option v (Some o))) None eq_refl))
+                               (vec_map
+                                  (fun a b0 : nat =>
+                                   derivₙₛ (Var (S + (V +{ n0}) \ Some o)%s) Z_ren a
+                                     (fun k : nat => Var (S + (V +{ n0}) \ Some o)%s ((v1) ̅ ¹ k)) b0) v0)) b
+                      end)) (vec_range0 (Z_model_data (S + V +{ n0})%s) (arm o)))) n)
+
+*)
+
+Tactic Notation "apply_both" tactic(tac) :=
+      etransitivity; [|symmetry; etransitivity] ; [tac | tac | ].
+
+
+Lemma unifier_spec_factors {V } (t u : T S V) c0 (W := cW c0)(ass := cass c0) c (ind : @unifier_spec _ t u c0 c)
+  : exists a , cass c = ass ∘a a 
+  (* is_unifier (t [ ass ]ₘ) (u [ ass ]ₘ) (m := ZModel (S + _)%s) (cass c) *)
+  with unifier_spec_vec_factors {V } (l : list nat)(v1 v2 : vec (T S V) l)
+       c0 (W := cW c0)(ass := cass c0) 
+       c (ind : @unifier_spec_vec _ _ v1 v2 c0 c):
+    exists a , cass c = ass ∘a a .
+{
+  subst ass.
+  destruct ind; cbn; try ((eexists;etransitivity;[|symmetry;apply assignation_comp_idl ];reflexivity)
+                         || (eexists; symmetry; apply assignation_comp_idr)).
+  - cbn in unifier_spec_vec_factors.
+    eapply unifier_spec_vec_factors.
+    eassumption.
+  - eexists.
+    reflexivity.
+  - eapply unifier_spec_factors.
+    eassumption.
+}
+{
+  subst ass.
+  destruct ind; cbn.
+  - eexists; symmetry; apply assignation_comp_idr.
+  - eapply unifier_spec_factors in H.
+    eapply unifier_spec_vec_factors in ind.
+    destruct H.
+    destruct ind.
+    rewrite H.
+    rewrite H0.
+    rewrite <- assignation_comp_assoc.
+    eexists.
+    reflexivity.
+}
+Qed.
+
+Lemma unifier_spec_preserve {V } (t u : T S V) c0 (W := cW c0)(ass := cass c0) c (ind : @unifier_spec _ t u c0 c)
+  :
+  forall t' u',
+  t' [ ass ]ₘ = u' [ ass ]ₘ ->
+  t' [  cass c ]ₘ = 
+  u' [  cass c ]ₘ.
+Proof.
+  apply unifier_spec_factors in ind.
+  destruct ind as [? eq].
+  intros.
+  rewrite eq.
+  rewrite <- 2!assignation_comp_msubst'.
+  f_equal.
+  assumption.
+Qed.
+  (* is_unifier (t [ ass ]ₘ) (u [ ass ]ₘ) (m := ZModel (S + _)%s) (cass c) *)
+(*
+  Lemma unifier_spec_vec_preserve {V } (l : list nat)(v1 v2 : vec (T S V) l)
+       c0 (W := cW c0)(ass := cass c0) 
+       c (ind : @unifier_spec_vec _ _ v1 v2 c0 c):
+  forall t' u',
+  t' [ ass ]ₘ = u' [ ass ]ₘ ->
+  t' [  cass c ]ₘ = 
+  u' [  cass c ]ₘ.
+    Proof.
+  apply unifier_spec_vec_factors in ind.
+  destruct ind as [? eq].
+  intros.
+  rewrite eq.
+  rewrite <- 2!assignation_comp_msubst'.
+  f_equal.
+  assumption.
+  Qed.
+*)
+  (*
+Proof.
+{
+  subst ass.
+  destruct ind; cbn; intros t' u'; rewrite ?msubst'_id; try congruence.
+  - cbn.
+    intro h.
+    eapply unifier_spec_vec_preserve; eassumption.
+  - rewrite <- !assignation_comp_msubst'.
+    cbn.
+    congruence.
+  - eapply unifier_spec_preserve.
+    eassumption.
+}
+{
+  subst ass.
+  destruct ind; cbn; intros t' u'; rewrite ?msubst'_id.
+  - congruence.
+  - cbn.
+    intro h.
+    eapply unifier_spec_preserve.
+    eassumption.
+    eapply unifier_spec_vec_preserve.
+    eassumption.
+    eassumption.
+}
+Qed.
+*)
+
+
+(*
+Fixpoint factors {A B B' : Type}(f : A -> B)(g : A -> B')
+  (hfg : forall t u,
+  f t = f u ->
+  g t = g u) C (lC : list C) (v1 : vec _ lC) {struct v1 }: forall (v2 : vec _ lC),
+    vec_map ( fun _ => f) v1 = vec_map ( fun _ => f) v2
+    -> vec_map ( fun _ => g) v1 = vec_map (fun _ => g) v2.
+  Admitted.
+*)
+
+Lemma unifier_spec_preserve_vec {V } (t u : T S V) c0 (W := cW c0)(ass := cass c0) c (ind : @unifier_spec _ t u c0 c)
+  
+   (l' : list nat) v1'  : forall v2' : vec (T S V) l', 
+     vec_map (fun _ t =>  t [  ass ]ₘ)  v1' =
+     vec_map (fun _ t => t [  ass ]ₘ)  v2'  -> 
+     vec_map (fun _ t =>  t [  cass c ]ₘ)  v1' =
+     vec_map (fun _ t => t [  cass c ]ₘ)  v2'.
+
+  apply unifier_spec_factors in ind.
+  destruct ind as [a eq].
+  intro v2'.
+  intro h.
+  assert (H : forall (v : vec (T S V) l'),   vec_map (fun (_ : nat) (t0 : T S V) => t0 [cass c ]ₘ) v =
+                                                vec_map (fun (_ : nat) t0 => t0 [ a ]ₘ)
+                                                (vec_map (fun (_ : nat) t0 => t0 [ cass c0 ]ₘ)
+                                                         v)
+            ).
+  {
+    intro v.
+    rewrite vec_map_map.
+    apply vec_map_ext.
+    intros.
+    rewrite eq.
+    symmetry.
+    apply assignation_comp_msubst'.
+  }
+  rewrite 2!H.
+  f_equal.
+  apply h.
+  Qed.
+  (*
+  assumption 
+  subst ass.
+  apply factors.
+  eapply unifier_spec_preserve.
+  eassumption.
+*)
 
 Lemma unifier_spec_correct {V } (t u : T S V) c0 (W := cW c0)(ass := cass c0) c (ind : @unifier_spec _ t u c0 c) :
   t [  cass c ]ₘ = 
@@ -1708,6 +2398,7 @@ Lemma unifier_spec_correct {V } (t u : T S V) c0 (W := cW c0)(ass := cass c0) c 
     f_equal.
     apply unifier_spec_vec_correct in H.
     apply H.
+    (*
   - destruct H.
     reflexivity.
   - (* candidate replace: same mvar *)
@@ -1717,17 +2408,21 @@ Lemma unifier_spec_correct {V } (t u : T S V) c0 (W := cW c0)(ass := cass c0) c 
     rewrite !vec_map_vecn.
     cbn.
     f_equal.
+    apply_both (apply (f_equal ( fun v => vec_map _ (l := _)(vec_map _ (l := _) v))); apply  replaced_vec_vec_map).
+    (*
     etransitivity;[|symmetry; etransitivity];
       try (apply (f_equal ( fun v => vec_map _ (l := _)(vec_map _ (l := _) v))); apply  replaced_vec_vec_map).
+*)
     rewrite !vec_map_map.
     cbn.
     unfold replaced_vec.
     destruct (o =m o); [|contradiction].
-    etransitivity; [|symmetry;etransitivity]; try apply vec_map_vecn.
+    apply_both (apply vec_map_vecn).
+    (* etransitivity; [|symmetry;etransitivity]; try apply vec_map_vecn. *)
     cbn.
 
-    etransitivity;[|symmetry;etransitivity];
-      try (
+    (* etransitivity;[|symmetry;etransitivity]; *)
+      apply_both (
     apply vec_map_ext;
     intros;
     unfold vec_to_ren;
@@ -1753,12 +2448,226 @@ Lemma unifier_spec_correct {V } (t u : T S V) c0 (W := cW c0)(ass := cass c0) c 
     eapply (f_equal (vec_map (fun _ => Var _) (l := _))) in h0.
     rewrite 2!vec_map_map in h0.
     exact h0.
+*)
+      - (* candidate replace bis: same mvar *)
+    rename X into commonPos.
+    cbn -[TMVar_replaced' assignation_comp].
+    cbn.
+    unfold assignation_instantiate.
+    rewrite (refl_deceq_true (Some o)).
+    cbn.
+    f_equal.
+    rewrite !vec_map_vecn.
+    rewrite !vec_map_map.
+    cbn.
+    rewrite !vec_map_vecn.
+    (* apply_both vec_map_vecn. *)
+    etransitivity; [|symmetry; etransitivity] ; try apply vec_map_vecn.
+    cbn.
+    apply vec_map_ext_In.
+    intros.
+    apply Z_in_fv_subst_ext.
+    intros n.
+    unfold vec_to_ren.
+    cbn.
+    unshelve erewrite (vec_nth_map'  _ _ (a := 0) );
+      [ eapply Var; shelve | |]; revgoals.
+    { cbn.
+      reflexivity.
+    }
+    cbn.
+    set (yy := vec_nth _ _  _).
+    eassert (hy : yy = _).
+    {
+      unfold yy.
+      apply (vec_to_ren_vec_range0 ( Z_model_data _)).
+    }
+    rewrite hy.
+    cbn.
+    intro hn.
+    inversion hn.
+    apply_both (apply (vec_nth_map' _ _ (a := 0)); reflexivity).
+    f_equal.
+    assert (inbv1 : Vec_In b v1). { eapply commonPos_Vec_In1; eassumption. }
+    assert (inbv2 : Vec_In b v2). { eapply commonPos_Vec_In2; eassumption. }
+    rewrite inverse_vec_is_inverse by assumption.
+    erewrite commonPos_Vec_inverse by eassumption.
+    symmetry.
+    apply inverse_vec_is_inverse.
+    assumption.
+
+  - (* different mvar *)
+
+    rename X into commonVal.
+    cbn -[TMVar_replaced' assignation_comp].
+    cbn -[eq_dec].
+    unfold assignation_instantiate.
+    unshelve erewrite (neq_negb_deceq_false (o' := Some o2)(o := Some o1)).
+    congruence.
+    unshelve rewrite (refl_deceq_true (Some o1)).
+    cbn -[eq_dec].
+    assert (neq_o2' : exist (fun v : option (Om V) => negb (deceq_option v (Some o1))) None eq_refl <> o2').
+    {
+      unfold o2'.
+      cbn.
+      congruence.
+    }
+    unshelve erewrite (neq_negb_deceq_false neq_o2').
+    cbn -[eq_dec].
+    f_equal.
+    rewrite !vec_map_vecn.
+    rewrite !vec_map_map.
+    cbn -[eq_dec].
+    rewrite !vec_map_vecn.
+    (* apply_both vec_map_vecn. *)
+    (* etransitivity; [|symmetry; etransitivity] ; try apply vec_map_vecn. *)
+    cbn -[eq_dec].
+    assert (eq_o2' :    exist (fun v : option (Om V) => v <>m Some o1) (Some o2)
+      (neq_negb_deceq
+         (fun H : Some o2 = Some o1 =>
+          False_ind False
+            (neq_o12 (f_equal (fun t : option (Om V) => match t with
+                                                        | Some H0 => H0
+                                                        | None => o1
+                                                        end) (eq_sym H))))) = o2').
+    {
+      unfold o2'.
+      cbn.
+      f_equal.
+      apply irrelevance_bool.
+    }
+    rewrite (deceq_eq_true eq_o2').
+    cbn -[eq_dec].
+    (*
+    assert (h0 : (
+       (exist (fun v : {v : option (Om V) | v <>m Some o1} => v <>m o2')
+          (exist (fun v : option (Om V) => negb (deceq_option v (Some o1))) None eq_refl) 
+          (neq_negb_deceq neq_o2'))
+
+                 )
+                   =
+                     (exist (fun v : {v : option (Om V) | negb (deceq_option v (Some o1))} => negb (subdeceq v o2'))
+          (exist (fun v : option (Om V) => negb (deceq_option v (Some o1))) None eq_refl) eq_refl)
+           ).
+    {
+    cbn.
+    f_equal.
+    Set Printing Implicit.
+    Check (neq_negb_deceq neq_o2').
+    }
+*)
+    set (e' := neq_negb_deceq neq_o2').
+    assert (eq_e' : e' = eq_refl (x := true)).
+    {
+      apply irrelevance_bool.
+    }
+    change (SMVar (S := S) (V := V +{ n0} \ _ \ _)
+       (exist (fun v : {v : option (Om V) | v <>m Some o1} => v <>m o2')
+          (exist (fun v : option (Om V) => negb (deceq_option v (Some o1))) None eq_refl) 
+          (neq_negb_deceq neq_o2')))
+           with (SMVar (S := S) (V := V +{ n0} \ _ \ _)
+       (exist (fun v : {v : option (Om V) | v <>m Some o1} => v <>m o2')
+          (exist (fun v : option (Om V) => negb (deceq_option v (Some o1))) None eq_refl) 
+          e')).
+    clearbody e'.
+    subst e'.
+    cbn -[eq_dec].
+    f_equal.
+    rewrite !vec_map_map.
+    cbn.
+    clear eq_o2'.
+    etransitivity; revgoals.
+    {
+      symmetry.
+    apply vec_map_vecn.
+    }
+    cbn.
+    apply vec_map_ext_In.
+    intros b bv0.
+    cbn.
+    unfold vec_to_ren.
+    etransitivity.
+    {
+      unshelve erewrite (vec_nth_map'  _ _ (a := 0) ); [ eapply Var; shelve | | cbn; reflexivity].
+      set (yy := vec_nth _ _  _).
+      eassert (hy : yy = _).
+      {
+        unfold yy.
+        apply (vec_to_ren_vec_range0 ( Z_model_data _)).
+      }
+      rewrite hy.
+      clear yy hy.
+      cbn.
+      set (yy := vec_nth _ _  _).
+      eassert (hy : yy = _).
+      {
+        unfold yy.
+        apply (vec_to_ren_vec_range0 ( Z_model_data _)).
+      }
+      rewrite hy.
+      clear yy hy.
+      cbn.
+      erewrite (vec_nth_map' _ _ (a := 0)); [ | reflexivity].
+      apply (f_equal (Var _)).
+      apply inverse_vec_is_inverse.
+      eapply commonVal_Vec_In1; eassumption.
+    }
+    etransitivity; revgoals.
+    {
+      symmetry.
+      set (vmap := vec_map (B := T S (V +{ n0 })) _ _ ).
+      eassert (eq_vmap : vmap = _).
+      {
+         apply vec_map_vecn.
+      }
+      clearbody vmap.
+      subst vmap.
+      cbn.
+      eassert (vecren := vec_to_ren_vec_range0( Z_model_data (S + (V +{ n0}) \ Some o1)%s) ((v2) ̅ ¹ b)).
+      unfold vec_to_ren in vecren.
+      cbn in vecren.
+      unshelve erewrite (vec_nth_map'  _ _ (a := 0) ); [eapply Var; exact (((v2) ̅ ¹ b)) |  |];revgoals.
+      {
+        cbn.
+        (* eassert (vecren := vec_to_ren_vec_range0( Z_model_data (S + (V +{ n0}) \ Some o1)%s) ((v2) ̅ ¹ b)). *)
+        rewrite vecren.
+        cbn.
+        reflexivity.
+      }
+      cbn.
+      set (yy := vec_nth _ _  _).
+      eassert (hy : yy = _).
+      {
+        unfold yy.
+        apply (vec_to_ren_vec_range0( Z_model_data (S + (V +{ n0}) )%s) ((v2) ̅ ¹ b)).
+      }
+      rewrite hy.
+      clear yy hy.
+      cbn.
+      set (yy := vec_nth _ _  _).
+      eassert (hy : yy = _).
+      {
+        unfold yy.
+        apply (vec_to_ren_vec_range0( Z_model_data (S + (V +{ n0}) \Some o1)%s) ((v2) ̅ ¹ b)).
+      }
+      rewrite hy.
+      clear yy hy.
+      cbn.
+      unshelve eapply (vec_nth_map' _ _ (a := 0)).
+      shelve.
+      reflexivity.
+    }
+    f_equal.
+    symmetry.
+    apply inverse_vec_is_inverse.
+    eapply commonVal_Vec_In2; eassumption.
   - apply unifier_spec_correct in ind.
     cbn.
     cbn in ind.
     rewrite <- 2! assignation_comp_msubst'.
     exact ind.
-  - hnf.
+  - (* instantiate *)
+    hnf.
     cbn -[remove_mvar].
     unfold assignation_instantiate at 1.
     rewrite (refl_deceq_true o).
@@ -1782,16 +2691,18 @@ Lemma unifier_spec_correct {V } (t u : T S V) c0 (W := cW c0)(ass := cass c0) c 
     (* rewrite vec_map_map. *)
     cbn.
     unfold vec_to_ren.
-    erewrite vec_nth_map'.
+    erewrite (vec_nth_map' _ _ (a := 0)).
 
     f_equal.
     apply inverse_vec_is_inverse.
     apply hufv.
     eapply In_fv_remove_mvar1.
     eassumption.
-    shelve.
     cbn.
     reflexivity.
+  - symmetry.
+    eapply  unifier_spec_correct.
+    eassumption.
     }
 {
   destruct ind.
@@ -1801,11 +2712,1093 @@ Lemma unifier_spec_correct {V } (t u : T S V) c0 (W := cW c0)(ass := cass c0) c 
   - specialize (unifier_spec_correct _ _ _ _ _ H).
     (* rewrite assignation_comp_assoc. *)
     apply unifier_spec_correct.
-  - generalize (unifier_spec_vec_correct _ _ _ _ _ _ ind).
-    revert H.
-    (* There we should prove that if the input c1 unfies, then the output c2 also does*)
-    admit.
+  -
+    (* generalize (unifier_spec_vec_correct _ _ _ _ _ _ ind). *)
+    eapply unifier_spec_preserve_vec.
+    eassumption.
+    apply (unifier_spec_vec_correct _ _ _ _ _ _ ind).
+}
+Qed.
+
+
+
+Lemma in_fv_vec_in {S'}(n : nat){p : nat}(v : nat ** p) :
+  In_fv_vec n (vec_map (fun _ => Var S') v) ->
+  Vec_In n v.
+Admitted.
+
+Lemma In_fv_msubst' {V : msignature} {W : msignature}(m := Z_model_data (S + W)%s)
+      (f : assignation V m)(t : T S V)(p : nat) : In_fv p t <-> In_fv p (t [ f ]ₘ).
+Admitted.
+
+(* not sure how to prove this.
+ Use the depth of the expression ? *)
+Lemma unified_notin_mvar {V } (t : T S V) {W}  (a : assignation V (Z_model_data (S + W)%s))
+         (o : Om V) v
+         (* (ht : forall v', vec_map (fun _ => msubst' a) v' = v -> t <> Op (S := S + V)%s (SMVar o) v')  *)
+         (ht : forall v',  t <> Op (S := S + V)%s (SMVar o) v') 
+      (ha : t [ a ]ₘ = a o v)  :  Notin_mvar o t.
+Admitted.
+
+Fixpoint build_vec_common_pos {B : Type}{eqb : EqDec B} (n1 : nat) (v1 : B ** n1) (v1' : B ** n1) : { n0 & B ** n0}.
+  Admitted.
+
+Lemma build_vec_common_pos_is_common_pos {B}{eqb : EqDec B}(n1 : nat) (v1 : B ** n1) (v1' : B ** n1)
+      : vec_common_pos (projT2 (build_vec_common_pos v1 v1')) v1 v1'.
+Admitted.
+
+Fixpoint build_vec_common_val {B : Type}{eqb : EqDec B} (n1 n1' : nat) (v1 : B ** n1) (v1' : B ** n1') : { n0 & B ** n0}.
+  Admitted.
+
+Lemma build_vec_common_val_is_common_val {B}{eqb : EqDec B}(n1 n1' : nat) (v1 : B ** n1) (v1' : B ** n1')
+      : vec_common_val v1 v1' (projT2 (build_vec_common_val v1 v1')).
+Admitted.
+
+(*
+This allows double recursion in the same time.
+TODO: maybe I can implement directly the algorithm as a fixpoint over
+this inductive type
+ *)
+Inductive valid_pair {V} : T S V -> T S V -> candidate V -> Type :=
+  vp_subst : forall c t u, valid_pair (t [ cass c]ₘ)(u [ cass c]ₘ) id_candidate
+                      -> valid_pair t u c
+  | vp_var_var : forall n n', valid_pair (Var _ n)(Var _ n') id_candidate
+  | vp_var_op : forall n o v, valid_pair (Var _ n)(Op (S := S + V)%s(SOp o) v) id_candidate
+  | vp_mvar_var : forall n o v, distinct v -> valid_pair (Op (S := S + V)%s(SMVar o) (vec_map (fun _ => Var _) v))(Var _ n) id_candidate
+  | vp_mvar_op : forall o v o' v', distinct v' -> valid_pair 
+                                          (Op (S := S + V)%s(SMVar o') (vec_map (fun _ => Var _) v'))
+                                          (Op (S := S + V)%s(SOp o) v)
+                                          id_candidate
+| vp_mvar_mvar : forall o v o' v',
+    distinct v -> distinct v' ->
+    valid_pair (Op (S := S + V)%s(SMVar o) (vec_map (fun _ => Var _) v))
+                                          (Op (S := S + V)%s(SMVar o') (vec_map (fun _ => Var _) v'))
+                                          id_candidate
+| vp_op_op : forall o o' (v : vec (T S V) (ar o))(v' : vec (T S V) (ar o')),
+    o <> o' ->
+    valid_pair (Op (S := S + V)%s (SOp o) v)
+               (Op (S := S + V)%s (SOp o') v')
+               id_candidate
+| vp_same_op : forall o (v v' : vec (T S V) (ar o)),
+    valid_pair_vec v v' id_candidate ->
+    valid_pair (Op (S := S + V)%s (SOp o) v)
+               (Op (S := S + V)%s (SOp o) v')
+               id_candidate
+
+  | vp_sym : forall c t u, valid_pair t u c -> valid_pair u t c
+with valid_pair_vec {V}  : forall (l : list nat), vec (T S V) l -> vec (T S V) l -> candidate V -> Type :=
+  | vp_nil_nil : forall c, valid_pair_vec NilV NilV c
+  (* | vp_cons_nil : forall l (v : vec (T S V) l) a b, valid_pair_vec (ConsV a b v) NilV *)
+  (* | vp_nil_cons : forall l (v : vec (T S V) l) a b, valid_pair_vec NilV (ConsV a b v). *)
+| vp_cons_cons : forall l (v : vec (T S V) l)(v' : vec (T S V) l) a b b' c0,
+                   (forall c, valid_pair b b' c) -> valid_pair_vec v v' c0 ->
+    valid_pair_vec (ConsV a b v) (ConsV a b' v') c0.
+(*
+Inductive valid_pair {V} : T S V -> T S V -> candidate V -> Type :=
+    vp_var_var : forall n n', valid_pair (Var _ n)(Var _ n')
+  | vp_var_op : forall n o v, valid_pair (Var _ n)(Op (S := S + V)%s(SOp o) v)
+  | vp_mvar_var : forall n o v, distinct v -> valid_pair (Op (S := S + V)%s(SMVar o) (vec_map (fun _ => Var _) v))(Var _ n)
+  | vp_mvar_op : forall o v o' v', distinct v' -> valid_pair 
+                                          (Op (S := S + V)%s(SMVar o') (vec_map (fun _ => Var _) v'))
+                                          (Op (S := S + V)%s(SOp o) v)
+| vp_mvar_mvar : forall o v o' v',
+    distinct v -> distinct v' ->
+    valid_pair (Op (S := S + V)%s(SMVar o) (vec_map (fun _ => Var _) v))
+                                          (Op (S := S + V)%s(SMVar o') (vec_map (fun _ => Var _) v'))
+| vp_op_op : forall o o' (v : vec (T S V) (ar o))(v' : vec (T S V) (ar o')),
+    o <> o' ->
+    valid_pair (Op (S := S + V)%s (SOp o) v)
+               (Op (S := S + V)%s (SOp o') v')
+| vp_same_op : forall o (v v' : vec (T S V) (ar o)),
+    valid_pair_vec v v' ->
+    valid_pair (Op (S := S + V)%s (SOp o) v)
+               (Op (S := S + V)%s (SOp o) v')
+
+  | vp_sym : forall t u, valid_pair t u -> valid_pair u t
+with valid_pair_vec {V}  : forall (l : list nat), vec (T S V) l -> vec (T S V) l -> Type :=
+  | vp_nil_nil : valid_pair_vec NilV NilV
+  (* | vp_cons_nil : forall l (v : vec (T S V) l) a b, valid_pair_vec (ConsV a b v) NilV *)
+  (* | vp_nil_cons : forall l (v : vec (T S V) l) a b, valid_pair_vec NilV (ConsV a b v). *)
+| vp_cons_cons : forall l (v : vec (T S V) l)(v' : vec (T S V) l) a b b',
+                   valid_pair b b' -> valid_pair_vec v v' ->
+    valid_pair_vec (ConsV a b v) (ConsV a b' v').
+*)
+
+Lemma aux V W (a : assignation _ (Z_model_data (S + W)%s)) :
+       forall n1 (v1 : _ ** n1),
+  vec_map
+    (fun (n0 : nat) (x : Z (S + W)%s) =>
+     x [derivₛ (Var (S + W)%s) Z_subst n0 (vec_to_ren (m := Z_model_data _) (vec_map (fun _ b : nat => Var (S + W)%s b) v1)) ]ₛ)
+    (vec_map (fun _ : nat => msubst' a) (vec_range0 (Z_model_data (S + V)%s) n1))
+    =   vec_map (fun _ : nat => Var (S + W)%s) v1 
+
+.
+          etransitivity;[ apply vec_map_vecn|].
+          cbn.
+          rewrite vec_map_map. 
+          cbn.
+          etransitivity;[ apply vec_map_mk|].
+          cbn.
+          apply vec_mk_nth0.
+          Qed.
+
+
+Arguments remove_mvar {V} t ov {h}.
+Arguments remove_mvar_vec {V} [l] v ov {h}.
+(*
+following theorem 7 of mcbride first order unification by structural recursion
+ *)
+Fixpoint unifier_spec_complete {V } (t u : T S V)
+                            (* (c0 := id_candidate) *)
+                            c0
+                            {W} (a : assignation _ (Z_model_data (S + W)%s))
+         (alaws : assignation_laws a)
+         (ha : t [ cass c0 ∘a a ]ₘ = u [ cass c0 ∘a a ]ₘ)  (valid : valid_pair t u c0) {struct valid} : exists c β δ', @unifier_spec _ t u c0 c
+                                                                                                                            (* because of the vec case, we can't seperate existence and factorisation of the given assignation a *)
+                                                                                                                            (*
+moreover, because of the substitution case (last case of MacBride), we need to prove factorisation of the
+output/input  at the same time, so this should be proved beforehand, before unifier_spec_factors
+                                                                                                                             *)
+    /\  cass c = cass c0 ∘a β /\ a = β ∘a δ' /\ assignation_laws δ'
+with unifier_spec_complete_vec {V }{l} (v1 : vec (T S V) l)(v2 : vec (T S V) l)
+                               (* (c0 := id_candidate) *)
+                               c0
+                               {W}  (a : assignation _ (Z_model_data (S + W)%s))
+         (alaws : assignation_laws a)
+         (ha : vec_map (fun _ => msubst'  (cass c0 ∘a a) ) v1 = vec_map (fun _ => msubst' (cass c0 ∘a a)) v2) (valid : valid_pair_vec v1 v2 c0) {struct valid} :
+  exists c β δ' , unifier_spec_vec v1 v2 c0 c
+    /\  cass c = cass c0 ∘a β /\ a = β ∘a δ' /\ assignation_laws δ'.
+  {
+    (*
+    cbn in ha.
+    rewrite (assignation_comp_idl (S := S)(V := V)) in ha.
+*)
+    (*
+  enough (h : forall t' u', valid_pair t' u' -> t' [ a ]ₘ = u' [ a ]ₘ ->  {c : candidate _ & unifier_spec t' u' id_candidate c}).
+  {
+    eexists.
+    apply applyass_spec.
+    refine (projT2 (h _ _ _ _ )).
+    rewrite 2!assignation_comp_msubst'.
+    assumption.
+  }
+*)
+  revert ha.
+  destruct valid; cbn.
+  - 
+    intro.
+    eapply unifier_spec_complete in valid0; try eassumption; revgoals.
+    {
+      cbn.
+      rewrite (assignation_comp_idl (S := S)(V := cW c)).
+      apply_both (eapply (assignation_comp_msubst' (m := Z_model_data (S + _)%s))).
+      congruence.
+    }
+    destruct valid0 as (c0 & β & δ' & un & fc0 & fa & lδ').
+    cbn in fc0.
+    rewrite (assignation_comp_idl (S := S)(V := cW c)) in fc0.
+    subst β.
+    repeat eexists.
+    + constructor.
+      eassumption.
+    + cbn.
+      reflexivity.
+    + eassumption.
+    + eassumption.
+  - intro ha.
+    injection ha.
+    intros ->.
+    do 3 eexists.
+    repeat split.
+    + econstructor.
+    + cbn.
+      symmetry.
+      apply assignation_comp_idl.
+    + symmetry.
+      apply assignation_comp_idl.
+    + assumption.
+  - discriminate.
+  - intro h.
+    rewrite vec_map_map in h.
+  (*   assert (hv : forall n1 (w : _ ** n1) w',  *)
+  (* vec_map *)
+  (*   (fun (n0 : nat) (x : Z (S + W)%s) => *)
+  (*    x [derivₛ (Var (S + W)%s) Z_subst n0 (vec_to_ren (vec_map (fun _ b : nat => Var (S + W)%s b) w)) ]ₛ) *)
+  (*   (vec_map (fun _ : nat => msubst' a) (vec_range0 (Z_model_data (S + V)%s) n1))  *)
+  (*    = w'). *)
+  (*                       (* (vec_map (fun _ : nat => Var (S + W)%s) w)). *) *)
+  (*                       (* (vec_map (fun _ : nat => Var (S + W)%s) w)). *) *)
+  (*   { *)
+  (*     intros n1 w. *)
+  (*     cbn. *)
+  (*     intro v0 *)
+      
+  (*   } *)
+    assert (hv : forall n1 (v1 : _ ** n1),
+  vec_map
+    (fun (n0 : nat) (x : Z (S + W)%s) =>
+     x [derivₛ (Var (S + W)%s) Z_subst n0 (vec_to_ren (m := Z_model_data _) (vec_map (fun _ b : nat => Var (S + W)%s b) v1)) ]ₛ)
+    (vec_map (fun _ : nat => msubst' a) (vec_range0 (Z_model_data (S + V)%s) n1))
+    =   vec_map (fun _ : nat => Var (S + W)%s) v1 
+
+).
+    {
+      apply aux.
+    }
+    eassert (h' :   a o (vec_map (fun _ : nat => Var (S + W)%s) v) = Var (S + W)%s n).
+    {
+          etransitivity;[|apply h].
+          etransitivity;[|symmetry; apply alaws].
+          f_equal.
+          symmetry.
+          apply hv.
+    }
+    (* unfold assignation_laws in alaws. *)
+    (* unfold an_assignation_laws in alaws. *)
+    (* unfold binding_condition in alaws. *)
+    do 2 eexists.
+    (* set (δ := assignation_omit a (o := o)). *)
+    refine (ex_intro _ ?[δ'] _).
+    repeat split.
+    + apply applyass_spec.
+      cbn.
+      rewrite vec_map_map.
+      cbn.
+      unshelve eapply instantiation_spec.
+      {
+        constructor.
+      }
+      intro p.
+      intro hin.
+      inversion hin.
+      subst.
+      (* if x ∈ fv (a v⃗), then x ∈ fv v
+Maybe show that x ∈ fv t <=> v [ x := x + 1] ≠ v
+       *)
+      unshelve eapply in_fv_vec_in; revgoals.
+      {
+        eapply assignation_fv.
+        + apply alaws.
+        + unshelve erewrite (_ : a o _ = Var _ n); [|constructor].
+          exact h'.
+      }
+    + cbn.
+      reflexivity.
+    + (* todo: think over it *)
+      cbn.
+      instantiate (δ' := assignation_omit a (o := o)).
+      apply assignation_ext.
+      intros o' v'.
+      cbn.
+      unfold assignation_raw_comp.
+      unfold mk_assignation_raw.
+      unfold mk_an_assignation_raw.
+      unfold assignation_instantiate.
+      destruct (o' =m o).
+      * subst o'.
+        cbn.
+         rewrite vec_to_ren_vec_range0.
+         enough (eqv' : v' = vec_map (fun _ x => x [ fun p => vec_to_ren v' (v ̅ ¹ p)  ]ₛ)
+                              (vec_map (fun _ : nat => Var (S + W)%s) v) ).
+         {
+           etransitivity.
+           {
+             eapply (f_equal (a o)).
+             exact eqv'.
+           }
+           etransitivity.
+           {
+             symmetry.
+             etransitivity; [ apply (alaws o)|].
+             rewrite vec_map_vecn.
+             cbn.
+             reflexivity.
+           }
+           cbn.
+           etransitivity.
+           {
+             apply (f_equal (fun x => x [ _ ]ₛ)).
+             exact h'.
+           }
+           cbn.
+           reflexivity.
+        }
+        rewrite vec_map_map.
+         cbn.
+         unfold vec_to_ren.
+         cbn.
+           symmetry.
+           eapply (inverse_vec_is_inverse2 v' _ (fun x => _ (v ̅ ¹ x))).
+      * cbn.
+        unfold assignation_omit.
+        cbn.
+        symmetry.
+        etransitivity;[apply alaws|].
+        eapply( f_equal (a o')).
+        cbn.
+        rewrite vec_map_map.
+        (* similar to the proof of hv *)
+        cbn.
+        rewrite vec_map_vecn.
+        cbn.
+        etransitivity;[ apply vec_map_mk|].
+        cbn.
+        apply vec_mk_nth0.
+    + apply assignation_omit_laws.
+      assumption.
+  - (* same proof as the previous one *)
+    rewrite vec_map_map.
+    cbn.
+    intro h.
+    eassert (h' : a o' (vec_map (fun _ : nat => Var (S + W)%s) v') = _).
+    {
+          etransitivity;[|apply h].
+          etransitivity;[|symmetry; apply alaws].
+          f_equal.
+          symmetry.
+          apply aux.
+    }
+    do 2 eexists.
+    refine (ex_intro _ ?[δ'] _).
+    repeat eexists.
+    + unshelve eapply instantiation_spec.
+      {
+        eapply unified_notin_mvar.
+        discriminate.
+        symmetry.
+        exact h.
+      }
+      intros p hin.
+      (* apply In_fv_Op in hin. *)
+      eapply in_fv_vec_in.
+      eapply assignation_fv;[apply alaws|].
+      unshelve erewrite (_ : a o' _ = _);[|exact h'|].
+      eapply In_fv_msubst' in hin.
+      cbn in hin.
+      exact hin.
+    + cbn.
+      symmetry.
+      apply assignation_comp_idl.
+    + cbn.
+      instantiate (δ' := assignation_omit a (o := o')).
+      apply assignation_ext.
+      intros o2 v2.
+      cbn.
+      unfold assignation_raw_comp.
+      unfold mk_assignation_raw.
+      unfold mk_an_assignation_raw.
+      unfold assignation_instantiate.
+      destruct (o2 =m o').
+      * subst o2.
+        cbn.
+         (* rewrite vec_to_ren_vec_range0. *)
+         enough (eqv' : v2 = vec_map (fun _ x => x [ fun p => vec_to_ren v2 (v' ̅ ¹ p)  ]ₛ)
+                              (vec_map (fun _ : nat => Var (S + W)%s) v') ).
+         {
+           etransitivity.
+           {
+             eapply (f_equal (a o')).
+             exact eqv'.
+           }
+           etransitivity.
+           {
+             symmetry.
+             etransitivity; [ apply (alaws o')|].
+             rewrite vec_map_vecn.
+             cbn.
+             reflexivity.
+           }
+           cbn.
+           etransitivity.
+           {
+             apply (f_equal (fun x => x [ _ ]ₛ)).
+             exact h'.
+           }
+           cbn.
+           rewrite remove_mvar_op.
+           cbn.
+           f_equal.
+           rewrite !vec_map_map.
+           cbn in a.
+           (* rewrite (assignation_comp_idl (m := Z_model_data (S + V)%s) a). *)
+           etransitivity.
+           {
+             apply vec_map_ext.
+             intros.
+             set  (a' :=  (id_assignation (m := Z_model_data (S + V)%s)∘a a)).
+             assert (eqa'' : a' = a).
+             {
+               unfold a'.
+               apply assignation_comp_idl.
+             }
+             rewrite eqa''.
+             reflexivity.
+           }
+           etransitivity; revgoals.
+           {
+             apply vec_map_ext.
+             intros.
+             symmetry.
+             etransitivity.
+             {
+             eapply (f_equal (fun x => x [ _ ]ₛ)).
+             etransitivity.
+             {
+             eapply (f_equal (fun x => (x [ _ ]ₘ : Z_model_data _) )).
+             etransitivity.
+             {
+               apply Z_subst_ext.
+               intro n.
+               etransitivity.
+               {
+               apply derivₙₛ_ext.
+               reflexivity.
+               intros.
+               eapply (vec_to_ren_vec_range0 (Z_model_data _)).
+               }
+               symmetry.
+               cbn.
+               eapply (var_derivₙ (var := Var _)).
+               reflexivity.
+             }
+             etransitivity.
+             {
+               eapply (f_equal (fun x => x [ _ ]ₛ)).
+               symmetry.
+               apply Z_subst_ext.
+               eapply (var_derivₙ (var := Var _)).
+               reflexivity.
+             }
+             rewrite Z_subst_subst.
+             cbn.
+             reflexivity.
+             }
+             symmetry.
+             apply (msubst'_ren ( m := Z_model_data _)).
+             }
+             cbn.
+             etransitivity; [apply Z_subst_subst|].
+             cbn.
+             apply Z_subst_ext.
+             intros.
+             rewrite derivₙₛ_derivₙ.
+             rewrite derivₙₛ_derivₙ.
+             reflexivity.
+
+           }
+           cbn.
+           set (ind := Notin_mvar_op _ ).
+           rewrite <- (remove_mvar_vec_assignation_incl  ind) at 1.
+           rewrite vec_map_map.
+           apply vec_map_ext.
+           intros.
+           f_equal.
+           etransitivity.
+           apply assignation_comp_msubst'.
+           unfold assignation_incl.
+           f_equal.
+           etransitivity.
+
+           symmetry.
+           eapply (assignation_omit_postcomp (m := Z_model_data _)).
+           f_equal.
+           apply assignation_comp_idl.
+         }
+        rewrite vec_map_map.
+         cbn.
+         unfold vec_to_ren.
+         cbn.
+           symmetry.
+           eapply (inverse_vec_is_inverse2 _ _ (fun x => _ (v' ̅ ¹ x))).
+      * cbn.
+        unfold assignation_omit.
+        cbn.
+        symmetry.
+        etransitivity;[apply alaws|].
+        f_equal.
+        rewrite vec_map_map.
+        (* similar to the proof of hv *)
+        cbn.
+        rewrite vec_map_vecn.
+        cbn.
+        etransitivity;[ apply vec_map_mk|].
+        cbn.
+        apply vec_mk_nth0.
+    + apply assignation_omit_laws.
+      assumption.
+  - destruct (o =m o').
+    + (* same mvar *)
+      subst o'.
+      intro h.
+      do 2 eexists.
+      refine (ex_intro _ ?[δ'] _).
+      repeat eexists.
+      * eapply same_mvar; try assumption.
+        apply build_vec_common_pos_is_common_pos; assumption.
+      * symmetry.
+        apply assignation_comp_idl.
+      * (* TODO: think over it *)
+        assert (d := ?δ').
+        cbn in d.
+        ICI
+        Check ?δ'.
+        admit.
+      * admit.
+    + (* different mvar *)
+      intro h.
+      repeat eexists.
+      * unshelve eapply different_mvar; revgoals.
+        apply build_vec_common_val_is_common_val.
+        assumption.
+      * symmetry.
+        apply assignation_comp_idl.
+      * admit.
+        (* TODO *)
+      * admit.
+  - cbn.
+    intro h.
+    injection h.
+    contradiction.
+  - intro eq.
+    assert (eq' : (vec_map (fun _ : nat => msubst' a) v) =  (vec_map (fun _ : nat => msubst' a) v')).
+    { admit. }
+    eapply unifier_spec_complete_vec in v0;[|eassumption|]; revgoals.
+    {
+      rewrite (assignation_comp_idl (S := S)(V := V)).
+      assumption.
+    }
+    destruct v0 as (c0 & β & δ' & un & fc0 & fa & δl).
+    repeat eexists.
+    + econstructor.
+      eassumption.
+    + symmetry.
+      apply assignation_comp_idl.
+    + rewrite fc0.
+      cbn.
+      rewrite (assignation_comp_idl (S := S)(V := V)).
+      eassumption.
+    + assumption.
+  - (* symmetric  *)
+    intro h.
+    eapply (unifier_spec_complete _ _ _ _ _ a alaws) in valid0; revgoals.
+    {
+      (* rewrite (assignation_comp_idl (S := S)(V := V)). *)
+      congruence.
+    }
+    destruct valid0 as (c0 & β & δ' & un & fc0 & fa & δl).
+    repeat eexists.
+    + apply sym_spec.
+      eassumption.
+    + eassumption.
+    + eassumption.
+    + eassumption.
+  }
+  {
+    (*
+        cbn in ha.
+    rewrite (assignation_comp_idl (S := S)(V := V)) in ha.
+*)
+
+    destruct valid.
+    - repeat eexists.
+      + constructor.
+      + symmetry.
+        apply assignation_comp_idr.
+      + symmetry.
+        apply assignation_comp_idl.
+      + assumption.
+    - cbn in ha.
+      eset (c := id_candidate ).
+      assert (eqb : b [cass c0 ∘a a ]ₘ = b' [cass c0 ∘a a ]ₘ).
+      {
+        admit.
+      }
+      assert (eqv :vec_map (fun _ : nat => msubst' (cass c0 ∘a a)) v = vec_map (fun _ : nat => msubst' (cass c0 ∘a a)) v').
+      {
+        admit.
+      }
+
+      eapply unifier_spec_complete_vec in valid0;[|apply alaws| exact eqv].
+      destruct valid0 as (c1 & β & δ' & un & fc1 & fa & δl).
+
+      (* assert (unc1' := unifier_spec_vec_factors unc1). *)
+      (* destruct unc1' as [a' eqa']. *)
+      specialize (v0 c1).
+      eapply unifier_spec_complete in v0; revgoals.
+      {
+        rewrite fc1.
+        rewrite fa  in eqb.
+        rewrite assignation_comp_assoc in eqb.
+        exact eqb.
+      }
+      { assumption. }
+      destruct v0 as (c2 & β' & δ'' & un' & fc2 & fa' & δl').
+      repeat eexists.
+      + econstructor.
+        * eassumption.
+        (*
+        eassert (h : _) ; [| exact h ].
+        {
+          admit.
+          (*
+        apply_both (apply vec_map_ext; intros
+                    ; rewrite (assignation_comp_idl (S := S)(V := V)) ; reflexivity
+                   ).
+
+        cbn.
+        symmetry.
+        exact eqv.
+*)
+       }
+*)
+      (* + eassert ( h := (projT2 (unifier_spec_complete _ _ _ _ _ _ alaws _ (v0 _)))). *)
+        *  eassumption.
+      + rewrite fc2.
+        rewrite fc1.
+        rewrite <- assignation_comp_assoc.
+        reflexivity.
+      + rewrite fa.
+        rewrite fa'.
+        rewrite assignation_comp_assoc.
+        reflexivity.
+      + assumption.
+  }
     Admitted.
+Fixpoint unifier_spec_complete {V } (t u : T S V)
+                            (* (c0 := id_candidate) *)
+                            c0
+                            {W} (a : assignation _ (Z_model_data (S + W)%s))
+         (alaws : assignation_laws a)
+      (ha : t [ cass c0 ∘a a ]ₘ = u [ cass c0 ∘a a ]ₘ)  (valid : valid_pair t u) {struct valid} : { c & @unifier_spec _ t u c0 c}
+with unifier_spec_complete_vec {V }{l} (v1 : vec (T S V) l)(v2 : vec (T S V) l)
+                               (* (c0 := id_candidate) *)
+                               c0
+                               {W}  (a : assignation _ (Z_model_data (S + W)%s))
+         (alaws : assignation_laws a)
+      (ha : vec_map (fun _ => msubst'  (cass c0 ∘a a) ) v1 = vec_map (fun _ => msubst' (cass c0 ∘a a)) v2) (valid : valid_pair_vec v1 v2) {struct valid} : { c & unifier_spec_vec v1 v2 c0 c}.
+  {
+    (*
+    cbn in ha.
+    rewrite (assignation_comp_idl (S := S)(V := V)) in ha.
+*)
+    (*
+  enough (h : forall t' u', valid_pair t' u' -> t' [ a ]ₘ = u' [ a ]ₘ ->  {c : candidate _ & unifier_spec t' u' id_candidate c}).
+  {
+    eexists.
+    apply applyass_spec.
+    refine (projT2 (h _ _ _ _ )).
+    rewrite 2!assignation_comp_msubst'.
+    assumption.
+  }
+*)
+  revert ha.
+  destruct valid; cbn.
+  - intro ha.
+    injection ha.
+    intros ->.
+    eexists.
+    econstructor.
+  - discriminate.
+  - intro h.
+    eexists.
+    apply applyass_spec.
+    cbn.
+    rewrite vec_map_map.
+    cbn.
+    unshelve eapply instantiation_spec.
+    {
+      constructor.
+    }
+    intro p.
+    intro hin.
+    inversion hin.
+    subst.
+    (* if x ∈ fv (a v⃗), then x ∈ fv v
+Maybe show that x ∈ fv t <=> v [ x := x + 1] ≠ v
+     *)
+    unshelve eapply in_fv_vec_in; revgoals.
+    {
+    eapply assignation_fv.
+    + apply alaws.
+    + rewrite vec_map_map in h.
+      cbn in h.
+      cbn.
+      unshelve erewrite (_ : a o _ = _);[| apply h | ].
+      constructor.
+      }
+  - (* same proof as the previous one *)
+    rewrite vec_map_map.
+    cbn.
+    intro h.
+    eexists.
+    unshelve eapply instantiation_spec.
+    {
+      eapply unified_notin_mvar.
+      discriminate.
+      symmetry.
+      exact h.
+    }
+    intros p hin.
+    (* apply In_fv_Op in hin. *)
+    eapply in_fv_vec_in.
+    eapply assignation_fv;[apply alaws|].
+    unshelve erewrite (_ : a o' _ = _);[| apply h | ].
+    eapply In_fv_msubst' in hin.
+    cbn in hin.
+    exact hin.
+  - destruct (o =m o').
+    + (* same mvar *)
+      subst o'.
+      intro h.
+      eexists.
+      eapply same_mvar; try assumption.
+      apply build_vec_common_pos_is_common_pos; assumption.
+    + (* different mvar *)
+      intro h.
+      eexists.
+      unshelve eapply different_mvar; revgoals.
+      apply build_vec_common_val_is_common_val.
+      assumption.
+  - cbn.
+    intro h.
+    injection h.
+    contradiction.
+  - 
+    intro eq.
+    assert (eq' : (vec_map (fun _ : nat => msubst' a) v) =  (vec_map (fun _ : nat => msubst' a) v')).
+    { admit. }
+    enough (h : { c & unifier_spec_vec v v' id_candidate c }).
+    {
+    eexists.
+    econstructor.
+    exact (projT2 h).
+    }
+    eapply unifier_spec_complete_vec; try eassumption.
+
+    rewrite (assignation_comp_idl (S := S)(V := V)).
+    assumption.
+  - (* symmetric  *)
+    intro h.
+    eapply (unifier_spec_complete _ _ _ _ a alaws) in valid0; revgoals.
+    {
+      rewrite (assignation_comp_idl (S := S)(V := V)).
+      congruence.
+    }
+    eexists.
+    apply sym_spec.
+    apply (projT2 valid0).
+  }
+  {
+        cbn in ha.
+    rewrite (assignation_comp_idl (S := S)(V := V)) in ha.
+
+    destruct valid.
+    - eexists.
+      constructor.
+    - cbn in ha.
+      assert (eqb : b [a ]ₘ = b' [a ]ₘ).
+      {
+        admit.
+      }
+      assert (eqv :vec_map (fun _ : nat => msubst' a) v = vec_map (fun _ : nat => msubst' a) v').
+      {
+        admit.
+      }
+
+      eexists.
+      econstructor.
+      + refine (projT2 (unifier_spec_complete_vec _ _ _ _ _ _ alaws _ _));[|assumption].
+        revert eqv.
+        shelve.
+        (*
+        eassert (h : _) ; [| exact h ].
+        {
+          admit.
+          (*
+        apply_both (apply vec_map_ext; intros
+                    ; rewrite (assignation_comp_idl (S := S)(V := V)) ; reflexivity
+                   ).
+
+        cbn.
+        symmetry.
+        exact eqv.
+*)
+       }
+*)
+      +  eassert ( h := (projT2 (unifier_spec_complete _ _ _ _ _ alaws _ v0))).
+         cbn in h.
+         eapply applyass_spec.
+        eapply unifier_spec_complete.
+  }
+    Admitted.
+
+Fixpoint unifier_spec_complete {V } (t u : T S V) {W}  (a : assignation V (Z_model_data (S + W)%s))
+         (alaws : assignation_laws a)
+      (ha : t [ a ]ₘ = u [ a ]ₘ) (valid : valid_pair t u) {struct valid} : { c & @unifier_spec _ t u id_candidate c}
+  with unifier_spec_complete_vec {V }{l} (v1 : vec (T S V) l)(v2 : vec (T S V) l) {W}  (a : assignation V (Z_model_data (S + W)%s))
+         (alaws : assignation_laws a)
+      (ha : vec_map (fun _ => msubst' a) v1 = vec_map (fun _ => msubst' a) v2) (valid : valid_pair_vec v1 v2) {struct valid} : { c & unifier_spec_vec v1 v2 id_candidate c}.
+  {
+  revert ha.
+  destruct valid; cbn.
+  - intro ha.
+    injection ha.
+    intros ->.
+    eexists.
+    econstructor.
+  - discriminate.
+  - intro h.
+    eexists.
+    unshelve eapply instantiation_spec.
+    {
+      constructor.
+    }
+    intro p.
+    intro hin.
+    inversion hin.
+    subst.
+    (* if x ∈ fv (a v⃗), then x ∈ fv v
+Maybe show that x ∈ fv t <=> v [ x := x + 1] ≠ v
+     *)
+    unshelve eapply in_fv_vec_in; revgoals.
+    {
+    eapply assignation_fv.
+    + apply alaws.
+    + rewrite vec_map_map in h.
+      cbn in h.
+      cbn.
+      unshelve erewrite (_ : a o _ = _);[| apply h | ].
+      constructor.
+      }
+  - (* same proof as the previous one *)
+    rewrite vec_map_map.
+    cbn.
+    intro h.
+    eexists.
+    unshelve eapply instantiation_spec.
+    {
+      eapply unified_notin_mvar.
+      discriminate.
+      symmetry.
+      exact h.
+    }
+    intros p hin.
+    (* apply In_fv_Op in hin. *)
+    eapply in_fv_vec_in.
+    eapply assignation_fv;[apply alaws|].
+    unshelve erewrite (_ : a o' _ = _);[| apply h | ].
+    eapply In_fv_msubst' in hin.
+    cbn in hin.
+    exact hin.
+  - destruct (o =m o').
+    + (* same mvar *)
+      subst o'.
+      intro h.
+      eexists.
+      eapply same_mvar; try assumption.
+      apply build_vec_common_pos_is_common_pos; assumption.
+    + (* different mvar *)
+      intro h.
+      eexists.
+      unshelve eapply different_mvar; revgoals.
+      apply build_vec_common_val_is_common_val.
+      assumption.
+  - cbn.
+    intro h.
+    injection h.
+    contradiction.
+  - 
+    intro eq.
+    assert (eq' : (vec_map (fun _ : nat => msubst' a) v) =  (vec_map (fun _ : nat => msubst' a) v')).
+    { admit. }
+    enough (h : { c & unifier_spec_vec v v' id_candidate c }).
+    {
+    eexists.
+    econstructor.
+    exact (projT2 h).
+    }
+    eapply unifier_spec_complete_vec; eassumption.
+  - (* symmetric  *)
+    intro h.
+    eapply (unifier_spec_complete _ _ _ _ a alaws) in valid0; [|congruence].
+    eexists.
+    apply sym_spec.
+    apply (projT2 valid0).
+  }
+  {
+    destruct valid.
+    - eexists.
+      constructor.
+    - cbn in ha.
+      assert (eqb : b [a ]ₘ = b' [a ]ₘ).
+      {
+        admit.
+      }
+      assert (eqv :vec_map (fun _ : nat => msubst' a) v = vec_map (fun _ : nat => msubst' a) v').
+      {
+        admit.
+      }
+
+      eexists.
+      econstructor.
+      + refine (projT2 (unifier_spec_complete_vec _ _ _ _ _ _ alaws _ _));[|assumption].
+        assumption.
+      +  eassert ( h := (projT2 (unifier_spec_complete _ _ _ _ _ alaws _ v0))).
+         cbn in h.
+         eapply applyass_spec.
+        eapply unifier_spec_complete.
+  }
+    Admitted.
+
+Fixpoint unifier_spec_general {V } (t u : T S V) {W}  (a : assignation V (Z_model_data (S + W)%s))
+         (ha : t [ a ]ₘ = u [ a ]ₘ)
+         {c}
+         (ind : unifier_spec t u id_candidate c)
+         {struct ind} : { a' : assignation _ _ | forall o v, a o v = (cass c ∘a a') (o := o) v}.
+  (* TODO *)
+Admitted.
+ 
+(*
+      rewrite <- h.
+    ICI
+    rewrite h in hin.
+    apply 
+    rewrite In_fv
+    econstructor.
+    discriminate.
+    contradiction.
+    
+  destruct t; cbn in ha.
+  - destruct u; cbn in ha.
+    cbn in ha.
+      c (ind : @unifier_spec _ t u c0 c) :
+  t [  cass c ]ₘ = 
+  u [  cass c ]ₘ
+  (* is_unifier (t [ ass ]ₘ) (u [ ass ]ₘ) (m := ZModel (S + _)%s) (cass c) *)
+*)
+(*
+  with unifier_spec_vec_complete {V } (l : list nat)(v1 v2 : vec (T S V) l)
+       c0 (W := cW c0)(ass := cass c0) 
+       c (ind : @unifier_spec_vec _ _ v1 v2 c0 c) :
+     vec_map (fun _ t =>  t [  cass c ]ₘ)  v1 =
+     vec_map (fun _ t => t [  cass c ]ₘ)  v2.
+*)
+
+(* ******************
+
+This version is like the previous one but with useless cases
+and without the symmetric case
+
+**************** *)
+Inductive unifier_spec  : forall V, T S V -> T S V -> forall (acc : candidate V) , candidate V -> Prop :=
+  var_spec : forall V n c, @unifier_spec V (Var _ n) (Var _ n) c c
+| sop_spec : forall V o v1 v2 c1 c2,
+    @unifier_spec_vec V _ v1 v2 c1 c2
+    ->
+    @unifier_spec V (Op (S := S + V)%s (SOp o) v1) (Op (S := S + V)%s (SOp o) v2) c1 c2
+                                     (* TODO correct *)
+                  (* TODO: remove *)
+| mvar_spec : forall V o (v1 v2 : vec nat (ar (s := S + V)%s(SMVar o))) c,
+    v1 = v2 ->
+    (* TODO: apply c to o *)
+    @unifier_spec V (Op (S := S + V)%s (SMVar o) (vec_map (fun _ => Var _)v1))
+                 (Op (S := S + V)%s (SMVar o) (vec_map (fun _ => Var _)v2))
+                 c c
+                 (* TODO: remove: same_mvar_bis is better since it does not require the definition of candidate_replace  *)
+| same_mvar : forall V o (v1 v2 : vec nat (ar (s := S + V)%s(SMVar o))) 
+                n0 v0, vec_common_pos (n0 := n0) v0 v1 v2 ->
+                       distinct v1 -> distinct v2 ->
+                       @unifier_spec V (Op (S := S + V)%s (SMVar o) (vec_map (fun _ => Var _)v1))
+                                     (Op (S := S + V)%s (SMVar o) (vec_map (fun _ => Var _)v2))
+                                     id_candidate
+                                     (candidate_replace (o := o)
+                                                (TMVar_replaced (vec_map (fun _ => Var _)v0)[ fun k =>  Var _ (v1 ̅ ¹ k) ]ₛ))
+| same_mvar_bis : forall V o (v1 v2 : vec nat (ar (s := S + V)%s(SMVar o))) 
+                n0 v0, vec_common_pos (n0 := n0) v0 v1 v2 ->
+                       distinct v1 -> distinct v2 ->
+                       @unifier_spec V (Op (S := S + V)%s (SMVar o) (vec_map (fun _ => Var _)v1))
+                                     (Op (S := S + V)%s (SMVar o) (vec_map (fun _ => Var _)v2))
+                                     id_candidate
+                                     (candidate_replace' (o := o)
+                                                (TMVar_replaced' (vec_map (fun _ => Var _)v0)[ fun k =>  Var _ (v1 ̅ ¹ k) ]ₛ))
+| different_mvar : forall V o1 o2 (neq_o12 : o1 <> o2)(v1 : vec nat (ar (s := S + V)%s(SMVar o1)))
+                     (v2 : vec nat (ar (s := S + V)%s(SMVar o2)))
+                     n0 v0
+                    (o2' := exist _ (Some o2) (neq_negb_deceq (neq_Some neq_o12)) : Om (V +{ n0 } \ Some o1))
+               , vec_common_val (n0 := n0) v1 v2 v0 ->
+                       (* distinct v1 -> distinct v2 -> *)
+                       @unifier_spec V (Op (S := S + V)%s (SMVar o1) (vec_map (fun _ => Var _)v1))
+                                     (Op (S := S + V)%s (SMVar o2) (vec_map (fun _ => Var _)v2))
+                                     id_candidate
+                                     (
+                                       id_candidate_ext n0
+                                        ∘c candidate_instantiate (V := V +{ n0 }) (o := Some o1)
+                                          (TMVar (V := V +{ n0 } \ Some o1)(o := exist _ None eq_refl)
+                                                (vec_map (fun _ p => Var _ (v1 ̅ ¹ p)) v0))
+                                        ∘c candidate_instantiate (V := V +{ n0 } \ Some o1)
+                                          (o := o2') 
+                                          (TMVar (V := V +{ n0 } \ Some o1 \ o2')(o := exist _ (exist _ None eq_refl) eq_refl)
+                                          (vec_map (fun _ p => Var _ (v2 ̅ ¹ p)) v0))
+                                     )
+                                     
+                                     (* (candidate_comp (r1 :=  *)
+                                     
+                                     (* candidate_replace (o := o1) *)
+                                     (*            (TMVar_replaced (vec_map (fun _ => Var _)v0)[ fun k =>  Var _ (v1 ̅ ¹ k) ]ₛ)) *)
+                                     (* (candidate_instantiate (o := o2) _) *)
+                                     (* ) *)
+
+(*
+1. m1[x1,..,xn] = m1[y1,..,yn]
+  m1 ↦ m3 whose arity the subset where xi = yi
+  m1[x1,..,xn] ↦ m3[]
+
+2. m1[x1,..,xn] = m2[y1,..,ym]
+  m1,m2 ↦ m3 whose arity the common intersection {x1,..,xn} ∩ {y1,..,ym}
+
+When metavariables are different, you can reorder those parameters in 2. but not in 1.
+ *)
+
+
+
+| applyass_spec : forall V t u c cf, @unifier_spec _ (t [ cass c ]ₘ) (u [ cass c ]ₘ) id_candidate cf
+                                            -> 
+                                              @unifier_spec V t u c (c ∘c cf)
+(* M[k1,...,kₙ] = t
+then M [u1,...,uₙ] = t [kᵢ ↦ uᵢ]
+Let us assume to start with that k1,...,kn = 0,..,n-1
+and maybe add an instantiation case that replace M[k1, ..., kn] with N[0,..,m]?
+ *)
+   (* ce qu il faut faire c'est construire un inverse (en tant que nat -> nat) de v (vecteur d'entiers) *)
+   (* et ensuite mk_assignation de t[v^-1] *)
+| instantiation_spec : forall V (c0 := id_candidate) o (n := arm o) (v : nat ** n)(* (v : nat ** arm o) *) (u : T S V)
+                         (hu : Notin_mvar o u)
+  (hufv : forall n, In_fv n u -> Vec_In n v), (* next_fv u <= n *)
+                          @unifier_spec V
+                                            (Op (S := S + V)%s (SMVar o) (vec_map (fun _ => Var _) v))
+                                            u
+                                            c0
+                                            (candidate_instantiate (remove_mvar hu [ fun k =>  Var _ (v ̅ ¹ k) ]ₛ))
+                                            (* (mk_assignation (m := ZModel (S + V \ o)) ) *)
+                                                           (* missing case: instantiation *)
+| instantiation_sym_spec : forall V (c0 := id_candidate) o (n := arm o) (v : nat ** n)(* (v : nat ** arm o) *) (u : T S V)
+                         (hu : Notin_mvar o u)
+  (hufv : forall n, In_fv n u -> Vec_In n v), (* next_fv u <= n *)
+                          @unifier_spec V
+                                            u
+                                            (Op (S := S + V)%s (SMVar o) (vec_map (fun _ => Var _) v))
+                                            c0
+                                            (candidate_instantiate (remove_mvar hu [ fun k =>  Var _ (v ̅ ¹ k) ]ₛ))
+
+with unifier_spec_vec : forall V (l : list nat), vec (T S V) l -> vec (T S V) l -> forall c : candidate V, candidate V -> Prop :=
+  NilV_spec : forall V c, @unifier_spec_vec V _ NilV NilV c c
+| ConsV_spec : forall V n l t1 t2 (v1 v2 : vec (T S V) l) c1  c1' c2, 
+                                                          (* do we need to take n into account? I think n *)
+                                        @unifier_spec_vec V _ v1 v2 c1 c1' ->
+                                        @unifier_spec V t1 t2 c1' c2 ->
+                                        @unifier_spec_vec V _ (ConsV n t1 v1) (ConsV n t2 v2) c1
+                                                         c2.
+
 (* ******************
 
 This version produces 
@@ -1820,7 +3813,7 @@ rather than T S V --> T S .. (see discussion belw)
                                                                      (* T S (cW acc) --> T S .. *)
                                                                      (* in mcbride, candidate V T S V --> T S .. *)
 Inductive unifier_spec  : forall V, T S V -> T S V -> forall (acc : candidate V) , candidate (cW acc) -> Prop :=
-  var_spec : forall V n c, @unifier_spec V (Var _ n) (Var _ n) c default_ass 
+  var_spec : forall V n c, @unifier_spec V (Var _ n) (Var _ n) c id_candidate 
 | sop_spec : forall V o v1 v2 c1 c2,
     @unifier_spec_vec V _ v1 v2 c1 c2
     ->
@@ -1831,7 +3824,7 @@ Inductive unifier_spec  : forall V, T S V -> T S V -> forall (acc : candidate V)
     (* TODO: apply c to o *)
     @unifier_spec V (Op (S := S + V)%s (SMVar o) (vec_map (fun _ => Var _)v1))
                  (Op (S := S + V)%s (SMVar o) (vec_map (fun _ => Var _)v2))
-                 c default_ass
+                 c id_candidate
 (*
 1. m1[x1,..,xn] = m1[y1,..,yn]
   m1 ↦ m3 whose arity the subset where xi = yi
@@ -1842,7 +3835,7 @@ Inductive unifier_spec  : forall V, T S V -> T S V -> forall (acc : candidate V)
 
 When metavariables are different, you can reorder those parameters in 2. but not in 1.
  *)
-| applyass_spec : forall V t u c cf, @unifier_spec _ (t [ cass c ]ₘ) (u [ cass c ]ₘ) default_ass cf
+| applyass_spec : forall V t u c cf, @unifier_spec _ (t [ cass c ]ₘ) (u [ cass c ]ₘ) id_candidate cf
                                             -> 
                                               @unifier_spec V t u c cf
                  (*
@@ -1860,7 +3853,7 @@ and maybe add an instantiation case that replace M[k1, ..., kn] with N[0,..,m]?
                                                            (* missing case: instantiation *)
 *)
 with unifier_spec_vec : forall V (l : list nat), vec (T S V) l -> vec (T S V) l -> forall c : candidate V, candidate (cW c) -> Prop :=
-  NilV_spec : forall V c, @unifier_spec_vec V _ NilV NilV c default_ass
+  NilV_spec : forall V c, @unifier_spec_vec V _ NilV NilV c id_candidate
 | ConsV_spec : forall V n l t1 t2 (v1 v2 : vec (T S V) l) c1  c1' c2, @unifier_spec_vec V _ v1 v2 c1 c1' ->
                                                           (* do we need to take n into account? I think n *)
                                         @unifier_spec V t1 t2 (candidate_comp c1') c2 ->
@@ -1950,7 +3943,7 @@ inductive principle is not strong enough
  *)
 
 Inductive unifier_spec {V} : T S V -> T S V -> candidate V -> Prop :=
-  var_spec : forall n, unifier_spec (Var _ n) (Var _ n) default_ass 
+  var_spec : forall n, unifier_spec (Var _ n) (Var _ n) id_candidate 
 | sop_spec : forall o v1 v2 c,
     unifier_spec_vec v1 v2 c
     ->
@@ -1960,7 +3953,7 @@ Inductive unifier_spec {V} : T S V -> T S V -> candidate V -> Prop :=
     v1 = v2 ->
     unifier_spec (Op (S := S + V)%s (SMVar o) (vec_map (fun _ => Var _)v1))
                  (Op (S := S + V)%s (SMVar o) (vec_map (fun _ => Var _)v1))
-                 default_ass
+                 id_candidate
 (* M[k1,...,kₙ] = t
 then M [u1,...,uₙ] = t [kᵢ ↦ uᵢ]
 Let us assume to start with that k1,...,kn = 0,..,n-1
@@ -1974,7 +3967,7 @@ and maybe add an instantiation case that replace M[k1, ..., kn] with N[0,..,m]?
                                             (* (mk_assignation (m := ZModel (S + V \ o)) ) *)
                                                            (* missing case: instantiation *)
 with unifier_spec_vec {V} : forall (l : list nat), vec (T S V) l -> vec (T S V) l -> candidate V -> Prop :=
-  NilV_spec : unifier_spec_vec NilV NilV default_ass
+  NilV_spec : unifier_spec_vec NilV NilV id_candidate
 | ConsV_spec : forall n l t1 t2 (v1 v2 : vec (T S V) l) c1 c2, unifier_spec_vec v1 v2 c1 ->
                                                           (* do we need to take n into account? I think n *)
                                         unifier_spec (t1 [ cass c1 ]ₘ) (t2 [ cass c1 ]ₘ) c2 ->
